[lean4] Reverting changes so signatures and examples work

lean4/Cdclt/examples/euf.lean
@@ -1,158 +1,157 @@
 import Cdclt.Euf
 
--- open proof
--- open proof.sort proof.Term
--- open rules eufRules
---
--- def U := atom (mkName "50")
--- def a₁ := const (mkName "100") U
--- def a₂ := const (mkName "101") U
--- def a₃ := const (mkName "102") U
--- def a₄ := const (mkName "103") U
--- def b₁ := const (mkName "104") U
--- def b₂ := const (mkName "105") U
--- def f₁ := const (mkName "106") (mkArrowN [U, U, U])
--- def f₂ := const (mkName "107") (mkArrowN [U, U, U])
--- def f₃ := const (mkName "108") (mkArrowN [U, U])
---
--- theorem binCong :
---   thHolds (mkEq a₁ a₂) → thHolds (mkEq b₁ b₂) → (thHolds (mkEq (mkApp (mkApp f₁ a₁) b₁) (mkApp (mkApp f₁ a₂) b₂))) :=
--- λ s0 : thHolds (mkEq a₁ a₂) =>
--- λ s1 : thHolds (mkEq b₁ b₂) =>
--- have s2 : thHolds (mkEq f₁ f₁) from refl
--- show (thHolds (mkEq (mkApp (mkApp f₁ a₁) b₁) (mkApp (mkApp f₁ a₂) b₂))) from cong (cong s2 s0) s1
---
---
--- def a1a2 := mkEq a₁ a₂
--- def f3a1 := (mkApp f₃ a₁)
--- def f3a2 := (mkApp f₃ a₂)
--- def f3a1f3a2 := mkEq f3a1 f3a2
--- def nf3a1f3a2 := mkNot f3a1f3a2
---
--- theorem test1 : thHolds a1a2 → thHolds nf3a1f3a2 → holds [] :=
--- λ s0 : thHolds a1a2 =>
--- λ s1 : thHolds nf3a1f3a2 =>
--- have s2 : thHolds (mkEq f₃ f₃) from refl
--- have s3 : thHolds f3a1f3a2 from cong s2 s0
--- have s4 : holds [mkNot a1a2, f3a1f3a2] from clOr (scope s0 s3)
--- show holds [] from R0 (R0 (clAssume s0) s4 a1a2) (clAssume s1) f3a1f3a2
---
--- /-
--- (SCOPE |:conclusion| (not (and (= a b) (or (not p3) (not (= (f a) (f b)))) p1 (or (not p1) (and p2 p3))))
---   (EQ_RESOLVE |:conclusion| false
---     (CHAIN_RESOLUTION |:conclusion| (not (= (f a) (f b)))
---       (ASSUME |:conclusion| (or (not p3) (not (= (f a) (f b)))) |:args| ((or (not p3) (not (= (f a) (f b))))))
---       (AND_ELIM |:conclusion| p3
---         (CHAIN_RESOLUTION |:conclusion| (and p2 p3)
---           (ASSUME |:conclusion| (or (not p1) (and p2 p3)) |:args| ((or (not p1) (and p2 p3))))
---           (ASSUME |:conclusion| p1 |:args| (p1)) |:args| (false p1))
---         |:args| (1))
---       |:args| (false p3))
---     (TRANS |:conclusion| (= (not (= (f a) (f b))) false)
---       (CONG |:conclusion| (= (not (= (f a) (f b))) (not (= (f b) (f b))))
---         (CONG |:conclusion| (= (= (f a) (f b)) (= (f b) (f b)))
---           (CONG |:conclusion| (= (f a) (f b))
---             (ASSUME |:conclusion| (= a b) |:args| ((= a b))) |:args| (23 f))
---           (REFL |:conclusion| (= (f b) (f b)) |:args| ((f b))) |:args| (6))
---         |:args| (17))
---       (TRANS |:conclusion| (= (not (= (f b) (f b))) false)
---         (CONG |:conclusion| (= (not (= (f b) (f b))) (not true))
---           (THEORY_REWRITE |:conclusion| (= (= (f b) (f b)) true) |:args| ((= (= (f b) (f b)) true) 2 5))
---           |:args| (17))
---         (THEORY_REWRITE |:conclusion| (= (not true) false) |:args| ((= (not true) false) 1 6)))))
---   |:args| ((= a b) (or (not p3) (not (= (f a) (f b)))) p1 (or (not p1) (and p2 p3))))
--- -/
---
--- def a := const  (mkName "1000") U
--- def b := const  (mkName "1001") U
--- def p₁ := const (mkName "1002") boolSort
--- def p₂ := const (mkName "1003") boolSort
--- def p₃ := const (mkName "1004") boolSort
--- def f := const  (mkName "1005") (mkArrowN [U, U])
--- def fa := mkApp f a
--- def fb := mkApp f b
---
--- def eqab := mkEq a b
--- def eqfafb := mkEq fa fb
--- def eqfbfb := mkEq fb fb
--- def eqfbfbtop := mkEq eqfbfb top
--- def neqfbfb := mkNot eqfbfb
--- def eqneqfbfbbot := mkEq neqfbfb bot
--- def eqeqfafbeqfbfb := mkEq eqfafb eqfbfb
--- def eqneqfafbneqfbfb := mkEq (mkNot eqfafb) (mkNot eqfbfb)
--- def neqfafb := mkNot eqfafb
--- def eqneqfafbbot := mkEq neqfafb bot
--- def np₁ := mkNot p₁
--- def np₃ := mkNot p₃
--- def andp₂p₃ := mkAnd p₂ p₃
--- def ornp₁andp₂p₃ := mkOr np₁ andp₂p₃
--- def ornp₃neqfafb := mkOr np₃ neqfafb
---
--- theorem simpleCongRw :
---   thHolds eqab → thHolds ornp₃neqfafb → thHolds p₁ → thHolds ornp₁andp₂p₃ → thHolds bot :=
--- λ s0 : thHolds eqab =>
--- λ s1 : thHolds ornp₃neqfafb =>
--- λ s2 : thHolds p₁ =>
--- λ s3 : thHolds ornp₁andp₂p₃ =>
---
--- have s4 : thHolds andp₂p₃ from thAssume (R1 (clOr s3) (clAssume s2) p₁)
--- have s5 : thHolds p₃ from andElim s4 1
--- have s6 : thHolds neqfafb from thAssume (R1 (clOr s1) (clAssume s5) p₃)
---
--- have s7 : thHolds eqfafb from cong refl s0
--- have s8 : thHolds eqeqfafbeqfbfb from cong (cong (@refl eqConst) s7) (@refl fb)
--- have s9 : thHolds eqneqfafbneqfbfb from cong (@refl notConst) s8
--- have s10 : thHolds (mkEq (mkNot top) bot) from thTrustValid
--- have s11 : thHolds eqfbfbtop from thTrustValid
--- have s12 : thHolds ((mkEq neqfbfb) (mkNot top)) from cong (@refl notConst) s11
--- have s13 : thHolds (mkEq neqfbfb bot) from trans s12 s10
--- have s14 : thHolds eqneqfafbbot from trans s9 s13
---
--- show thHolds bot from eqResolve s6 s14
---
--- /-
--- (SCOPE |:conclusion| (not (and (= a b) (or (not p3) (not (= (f a) (f b)))) p1 (or (not p1) (and p2 p3))))
---   (CHAIN_RESOLUTION |:conclusion| false
---     (REORDERING |:conclusion| (or (= (f a) (f b)) (not (= a b)))
---       (IMPLIES_ELIM |:conclusion| (or (not (= a b)) (= (f a) (f b)))
---         (SCOPE |:conclusion| (=> (= a b) (= (f a) (f b)))
---           (CONG |:conclusion| (= (f a) (f b))
---             (SYMM |:conclusion| (= a b)
---               (SYMM |:conclusion| (= b a)
---                 (ASSUME |:conclusion| (= a b) |:args| ((= a b))))) |:args| (23 f))
---           |:args| ((= a b))))
---       |:args| ((or (= (f a) (f b)) (not (= a b)))))
---     (CHAIN_RESOLUTION |:conclusion| (not (= (f a) (f b)))
---       (ASSUME |:conclusion| (or (not p3) (not (= (f a) (f b)))) |:args| ((or (not p3) (not (= (f a) (f b))))))
---       (CHAIN_RESOLUTION |:conclusion| p3
---         (REORDERING |:conclusion| (or p3 (not (and p2 p3)))
---           (CNF_AND_POS |:conclusion| (or (not (and p2 p3)) p3) |:args| ((and p2 p3) 1)) |:args| ((or p3 (not (and p2 p3)))))
---         (CHAIN_RESOLUTION |:conclusion| (and p2 p3)
---           (ASSUME |:conclusion| (or (not p1) (and p2 p3)) |:args| ((or (not p1) (and p2 p3))))
---           (ASSUME |:conclusion| p1 |:args| (p1)) |:args| (false p1))
---         |:args| (false (and p2 p3)))
---       |:args| (false p3))
---     (ASSUME |:conclusion| (= a b) |:args| ((= a b)))
---     |:args| (true (= (f a) (f b)) false (= a b)))
---   |:args| ((= a b) (or (not p3) (not (= (f a) (f b)))) p1 (or (not p1) (and p2 p3))))
--- -/
---
--- theorem simpleCong :
---   thHolds eqab → thHolds ornp₃neqfafb → thHolds p₁ → thHolds ornp₁andp₂p₃ → holds [] :=
--- λ s0 : thHolds eqab =>
--- λ s1 : thHolds ornp₃neqfafb =>
--- λ s2 : thHolds p₁ =>
--- λ s3 : thHolds ornp₁andp₂p₃ =>
--- have s4 : thHolds (mkEq b a) from symm s0
--- have s5 : thHolds eqab from symm s4
--- have s6 : thHolds eqfafb from cong (@refl f) s5
--- have s7 : holds [mkNot eqab, eqfafb] from clOr (scope s0 s6)
--- have s8 : holds [eqfafb, mkNot eqab] from reorder [1,0] s7
---
--- have s9 : holds [andp₂p₃] from R1 (clOr s3) (clAssume s2) p₁
--- have s10 : holds [mkNot andp₂p₃, p₃] from @cnfAndPos [p₂, p₃] 1
--- have s11 : holds [p₃, mkNot andp₂p₃] from reorder [1,0] s10
--- have s12 : holds [p₃] from R1 s11 s9 andp₂p₃
--- have s13 : holds [neqfafb] from R1 (clOr s1) s12 p₃
---
--- show holds [] from R1 s13 (R0 (clAssume s0) s8 eqab) eqfafb
+open proof
+open proof.sort proof.term
+open rules eufRules
+
+def U := atom 50
+def a₁ := const 100 U
+def a₂ := const 101 U
+def a₃ := const 102 U
+def a₄ := const 103 U
+def b₁ := const 104 U
+def b₂ := const 105 U
+def f₁ := const 106 (mkArrowN [U, U, U])
+def f₂ := const 107 (mkArrowN [U, U, U])
+def f₃ := const 108 (mkArrowN [U, U])
+
+theorem binCong :
+  thHolds (mkEq a₁ a₂) → thHolds (mkEq b₁ b₂) → (thHolds (mkEq (mkApp (mkApp f₁ a₁) b₁) (mkApp (mkApp f₁ a₂) b₂))) :=
+λ s0 : thHolds (mkEq a₁ a₂) =>
+λ s1 : thHolds (mkEq b₁ b₂) =>
+have s2 : thHolds (mkEq f₁ f₁) from refl
+show (thHolds (mkEq (mkApp (mkApp f₁ a₁) b₁) (mkApp (mkApp f₁ a₂) b₂))) from cong (cong s2 s0) s1
+
+def a1a2 := mkEq a₁ a₂
+def f3a1 := (mkApp f₃ a₁)
+def f3a2 := (mkApp f₃ a₂)
+def f3a1f3a2 := mkEq f3a1 f3a2
+def nf3a1f3a2 := mkNot f3a1f3a2
+
+theorem test1 : thHolds a1a2 → thHolds nf3a1f3a2 → holds [] :=
+λ s0 : thHolds a1a2 =>
+λ s1 : thHolds nf3a1f3a2 =>
+have s2 : thHolds (mkEq f₃ f₃) from refl
+have s3 : thHolds f3a1f3a2 from cong s2 s0
+have s4 : holds [mkNot a1a2, f3a1f3a2] from clOr (scope s0 s3)
+show holds [] from R0 (R0 (clAssume s0) s4 a1a2) (clAssume s1) f3a1f3a2
+
+/-
+(SCOPE |:conclusion| (not (and (= a b) (or (not p3) (not (= (f a) (f b)))) p1 (or (not p1) (and p2 p3))))
+  (EQ_RESOLVE |:conclusion| false
+    (CHAIN_RESOLUTION |:conclusion| (not (= (f a) (f b)))
+      (ASSUME |:conclusion| (or (not p3) (not (= (f a) (f b)))) |:args| ((or (not p3) (not (= (f a) (f b))))))
+      (AND_ELIM |:conclusion| p3
+        (CHAIN_RESOLUTION |:conclusion| (and p2 p3)
+          (ASSUME |:conclusion| (or (not p1) (and p2 p3)) |:args| ((or (not p1) (and p2 p3))))
+          (ASSUME |:conclusion| p1 |:args| (p1)) |:args| (false p1))
+        |:args| (1))
+      |:args| (false p3))
+    (TRANS |:conclusion| (= (not (= (f a) (f b))) false)
+      (CONG |:conclusion| (= (not (= (f a) (f b))) (not (= (f b) (f b))))
+        (CONG |:conclusion| (= (= (f a) (f b)) (= (f b) (f b)))
+          (CONG |:conclusion| (= (f a) (f b))
+            (ASSUME |:conclusion| (= a b) |:args| ((= a b))) |:args| (23 f))
+          (REFL |:conclusion| (= (f b) (f b)) |:args| ((f b))) |:args| (6))
+        |:args| (17))
+      (TRANS |:conclusion| (= (not (= (f b) (f b))) false)
+        (CONG |:conclusion| (= (not (= (f b) (f b))) (not true))
+          (THEORY_REWRITE |:conclusion| (= (= (f b) (f b)) true) |:args| ((= (= (f b) (f b)) true) 2 5))
+          |:args| (17))
+        (THEORY_REWRITE |:conclusion| (= (not true) false) |:args| ((= (not true) false) 1 6)))))
+  |:args| ((= a b) (or (not p3) (not (= (f a) (f b)))) p1 (or (not p1) (and p2 p3))))
+-/
+
+def a := const 1000 U
+def b := const 1001 U
+def p₁ := const 1002 boolSort
+def p₂ := const 1003 boolSort
+def p₃ := const 1004 boolSort
+def f := const 1005 (mkArrowN [U, U])
+def fa := mkApp f a
+def fb := mkApp f b
+
+def eqab := mkEq a b
+def eqfafb := mkEq fa fb
+def eqfbfb := mkEq fb fb
+def eqfbfbtop := mkEq eqfbfb top
+def neqfbfb := mkNot eqfbfb
+def eqneqfbfbbot := mkEq neqfbfb bot
+def eqeqfafbeqfbfb := mkEq eqfafb eqfbfb
+def eqneqfafbneqfbfb := mkEq (mkNot eqfafb) (mkNot eqfbfb)
+def neqfafb := mkNot eqfafb
+def eqneqfafbbot := mkEq neqfafb bot
+def np₁ := mkNot p₁
+def np₃ := mkNot p₃
+def andp₂p₃ := mkAnd p₂ p₃
+def ornp₁andp₂p₃ := mkOr np₁ andp₂p₃
+def ornp₃neqfafb := mkOr np₃ neqfafb
+
+theorem simpleCongRw :
+  thHolds eqab → thHolds ornp₃neqfafb → thHolds p₁ → thHolds ornp₁andp₂p₃ → thHolds bot :=
+λ s0 : thHolds eqab =>
+λ s1 : thHolds ornp₃neqfafb =>
+λ s2 : thHolds p₁ =>
+λ s3 : thHolds ornp₁andp₂p₃ =>
+
+have s4 : thHolds andp₂p₃ from thAssume (R1 (clOr s3) (clAssume s2) p₁)
+have s5 : thHolds p₃ from andElim s4 1
+have s6 : thHolds neqfafb from thAssume (R1 (clOr s1) (clAssume s5) p₃)
+
+have s7 : thHolds eqfafb from cong refl s0
+have s8 : thHolds eqeqfafbeqfbfb from cong (cong (@refl eqConst) s7) (@refl fb)
+have s9 : thHolds eqneqfafbneqfbfb from cong (@refl notConst) s8
+have s10 : thHolds (mkEq (mkNot top) bot) from thTrustValid
+have s11 : thHolds eqfbfbtop from thTrustValid
+have s12 : thHolds ((mkEq neqfbfb) (mkNot top)) from cong (@refl notConst) s11
+have s13 : thHolds (mkEq neqfbfb bot) from trans s12 s10
+have s14 : thHolds eqneqfafbbot from trans s9 s13
+
+show thHolds bot from eqResolve s6 s14
+
+/-
+(SCOPE |:conclusion| (not (and (= a b) (or (not p3) (not (= (f a) (f b)))) p1 (or (not p1) (and p2 p3))))
+  (CHAIN_RESOLUTION |:conclusion| false
+    (REORDERING |:conclusion| (or (= (f a) (f b)) (not (= a b)))
+      (IMPLIES_ELIM |:conclusion| (or (not (= a b)) (= (f a) (f b)))
+        (SCOPE |:conclusion| (=> (= a b) (= (f a) (f b)))
+          (CONG |:conclusion| (= (f a) (f b))
+            (SYMM |:conclusion| (= a b)
+              (SYMM |:conclusion| (= b a)
+                (ASSUME |:conclusion| (= a b) |:args| ((= a b))))) |:args| (23 f))
+          |:args| ((= a b))))
+      |:args| ((or (= (f a) (f b)) (not (= a b)))))
+    (CHAIN_RESOLUTION |:conclusion| (not (= (f a) (f b)))
+      (ASSUME |:conclusion| (or (not p3) (not (= (f a) (f b)))) |:args| ((or (not p3) (not (= (f a) (f b))))))
+      (CHAIN_RESOLUTION |:conclusion| p3
+        (REORDERING |:conclusion| (or p3 (not (and p2 p3)))
+          (CNF_AND_POS |:conclusion| (or (not (and p2 p3)) p3) |:args| ((and p2 p3) 1)) |:args| ((or p3 (not (and p2 p3)))))
+        (CHAIN_RESOLUTION |:conclusion| (and p2 p3)
+          (ASSUME |:conclusion| (or (not p1) (and p2 p3)) |:args| ((or (not p1) (and p2 p3))))
+          (ASSUME |:conclusion| p1 |:args| (p1)) |:args| (false p1))
+        |:args| (false (and p2 p3)))
+      |:args| (false p3))
+    (ASSUME |:conclusion| (= a b) |:args| ((= a b)))
+    |:args| (true (= (f a) (f b)) false (= a b)))
+  |:args| ((= a b) (or (not p3) (not (= (f a) (f b)))) p1 (or (not p1) (and p2 p3))))
+-/
+
+theorem simpleCong :
+  thHolds eqab → thHolds ornp₃neqfafb → thHolds p₁ → thHolds ornp₁andp₂p₃ → holds [] :=
+λ s0 : thHolds eqab =>
+λ s1 : thHolds ornp₃neqfafb =>
+λ s2 : thHolds p₁ =>
+λ s3 : thHolds ornp₁andp₂p₃ =>
+have s4 : thHolds (mkEq b a) from symm s0
+have s5 : thHolds eqab from symm s4
+have s6 : thHolds eqfafb from cong (@refl f) s5
+have s7 : holds [mkNot eqab, eqfafb] from clOr (scope s0 s6)
+have s8 : holds [eqfafb, mkNot eqab] from reorder [1,0] s7
+
+have s9 : holds [andp₂p₃] from R1 (clOr s3) (clAssume s2) p₁
+have s10 : holds [mkNot andp₂p₃, p₃] from @cnfAndPos [p₂, p₃] 1
+have s11 : holds [p₃, mkNot andp₂p₃] from reorder [1,0] s10
+have s12 : holds [p₃] from R1 s11 s9 andp₂p₃
+have s13 : holds [neqfafb] from R1 (clOr s1) s12 p₃
+
+show holds [] from R1 s13 (R0 (clAssume s0) s8 eqab) eqfafb
