lean4/Cdclt/BV.lean
@@ -3,12 +3,12 @@ import Cdclt.Boolean
 import Cdclt.TermEval
 
 open proof
-open proof.sort proof.Term
-open rules
+open proof.sort proof.term
+open rules 
 
 namespace proof
 
-namespace Term
+namespace term
 
 -- bit-vector sort definition
 @[matchPattern] def bvSort := sort.bv
@@ -27,18 +27,18 @@ MSB ... LSB
 
 /- mkBitOf bv n returns the nth element
    of bv if it exists; none otherwise -/
-def mkBitOf : OptionM Term → OptionM Term → OptionM Term :=
-λ ot₁ ot₂ =>
-  ot₁ >>= λ t₁ => ot₂ >>= λ t₂ =>
+def mkBitOf : Option term → Option term → Option term :=
+λ ot₁ ot₂ => 
+  ot₁ >>= λ t₁ => ot₂ >>= λ t₂ => 
   sortOf t₁ >>= λ s₁ => sortOf t₂ >>= λ s₂ =>
 match (s₁, s₂) with
 | (bv n, intSort) =>
   match t₂ with
   -- integer index has to be an in-range value
-  | val (Value.integer i) _ => if (i >= 0 ∧ i < n) then
+  | val (value.integer i) _ => if (i >= 0 ∧ i < n) then
     (match t₁ with
     -- BV can be a constant
-    | val (Value.bitvec l) _ =>
+    | val (value.bitvec l) _ =>
         match (List.get? (Int.toNat i) l) with
         | some b => if b then top else bot
         | none => none
@@ -46,73 +46,73 @@ match (s₁, s₂) with
     | _ => bitOf n t₁ t₂) else none
   | _ => none
 | (_, _) => none
-#check mkBitOf (val (Value.bitvec [true, false, true, false]) (bv 4)) (val (Value.integer 0) intSort)
-#check mkBitOf (val (Value.bitvec [true, false, true, false]) (bv 4)) (val (Value.integer 1) intSort)
-#check mkBitOf (val (Value.bitvec [true, false, true, false]) (bv 4)) (val (Value.integer 4) intSort)
-#check mkBitOf (const (mkName "x") (bv 4)) (val (Value.integer 0) intSort)
-#check mkBitOf (const (mkName "x") (bv 4)) (val (Value.integer 1) intSort)
-#check mkBitOf (const (mkName "x") (bv 4)) (val (Value.integer 4) intSort)
+#eval mkBitOf (val (value.bitvec [true, false, true, false]) (bv 4)) (val (value.integer 0) intSort)
+#eval mkBitOf (val (value.bitvec [true, false, true, false]) (bv 4)) (val (value.integer 1) intSort)
+#eval mkBitOf (val (value.bitvec [true, false, true, false]) (bv 4)) (val (value.integer 4) intSort)
+#eval mkBitOf (const 21 (bv 4)) (val (value.integer 0) intSort)
+#eval mkBitOf (const 21 (bv 4)) (val (value.integer 1) intSort)
+#eval mkBitOf (const 21 (bv 4)) (val (value.integer 4) intSort)
 
 /- bitOfN t n
    bit-blasts a BV constant or variable.
-   t is the BV Term and n is its length.
+   t is the BV term and n is its length.
    bitOfN t n returns a list of length n
-   with option Terms representing each bit.
+   with option terms representing each bit.
 -/
-def bitOfNAux : Term → Nat → Nat → List (OptionM Term)
+def bitOfNAux : term → Nat → Nat → List (Option term)
 | t, 0, _ => []
-| t, (n₁+1), n₂ => (mkBitOf t (val (Value.integer (Int.ofNat (n₂ - n₁ - 1))) intSort))
+| t, (n₁+1), n₂ => (mkBitOf t (val (value.integer (Int.ofNat (n₂ - n₁ - 1))) intSort)) 
                     :: (bitOfNAux t n₁ n₂)
 
-def bitOfN : Term → Nat → List (OptionM Term) :=
+def bitOfN : term → Nat → List (Option term) :=
   λ t n => bitOfNAux t n n
 
-#check bitOfN (const (mkName "x") (bv 4)) 4
-#check bitOfN (val (Value.bitvec [true, true, true, false]) (bv 4)) 4
-/- The following bad calls create bad bit-blasted Terms
+#eval bitOfN (const 21 (bv 4)) 4
+#eval bitOfN (val (value.bitvec [true, true, true, false]) (bv 4)) 4
+/- The following bad calls create bad bit-blasted terms
    because the nat argument to bitOfN and the length
-   of the BV Term don't match.-/
-#check bitOfN (const (mkName "x") (bv 3)) 4
-#check bitOfN (val (Value.bitvec [true, true, true, false]) (bv 4)) 3
+   of the BV term don't match.-/
+#eval bitOfN (const 21 (bv 3)) 4
+#eval bitOfN (val (value.bitvec [true, true, true, false]) (bv 4)) 3
 
 
 /- bitOfNRev works like bitOfN but in reverse -/
-def bitOfNRevAux : Term → Nat → List (OptionM Term)
-| t, 0 => (mkBitOf t (val (Value.integer (Int.ofNat 0)) intSort)) :: []
-| t, (n + 1) => (mkBitOf t (val (Value.integer (Int.ofNat (n + 1))) intSort))
+def bitOfNRevAux : term → Nat → List (Option term)
+| t, 0 => (mkBitOf t (val (value.integer (Int.ofNat 0)) intSort)) :: []
+| t, (n + 1) => (mkBitOf t (val (value.integer (Int.ofNat (n + 1))) intSort))
                     :: (bitOfNRevAux t n)
 
-def bitOfNRev : Term → Nat → List (OptionM Term) :=
+def bitOfNRev : term → Nat → List (Option term) :=
   λ t n => bitOfNRevAux t (n-1)
 
-#check bitOfNRev (const (mkName "x") (bv 4)) 4
-#check bitOfNRev (val (Value.bitvec [true, true, true, false]) (bv 4)) 4
-/- The following bad calls create bad bit-blasted Terms
+#eval bitOfNRev (const 21 (bv 4)) 4
+#eval bitOfNRev (val (value.bitvec [true, true, true, false]) (bv 4)) 4
+/- The following bad calls create bad bit-blasted terms
    because the nat argument to bitOfN and the length
-   of the BV Term don't match.-/
-#check bitOfNRev (const (mkName "x") (bv 3)) 4
-#check bitOfNRev (val (Value.bitvec [true, true, true, false]) (bv 4)) 3
+   of the BV term don't match.-/
+#eval bitOfNRev (const 21 (bv 3)) 4
+#eval bitOfNRev (val (value.bitvec [true, true, true, false]) (bv 4)) 3
 
 
 --------------------------------------- Bitwise Operators ---------------------------------------
 
 /-
 mkBbT l
-Construct a BV Term that is a bbT (bit-blasted Term)
+Construct a BV term that is a bbT (bit-blasted term) 
 of the bools in l
 -/
-@[matchPattern] def mkBbT (l : List (OptionM Term)) : OptionM Term :=
-  mkAppN (bbTConst (List.length l)) l
+@[matchPattern] def mkBbT (l : List (Option term)) : Option term :=
+  mkAppN (bbT (List.length l)) l
 
-#check mkBbT ([some top, some top, some top, some top])
+#eval mkBbT ([some top, some top, some top, some top])
 
 /-
 checkBinaryBV ot₁ ot₂ constr
 If ot₁ and ot₂ are BVs of the same length, then
 construct a bitwise op of (constr ot₁ ot₂)
 -/
-def checkBinaryBV : OptionM Term → OptionM Term →
-  (Nat → Term → Term → Term) → OptionM Term :=
+def checkBinaryBV : Option term → Option term →
+  (Nat → term → term → term) → Option term :=
   λ ot₁ ot₂ constr =>
     ot₁ >>= λ t₁ => ot₂ >>= λ t₂ =>
     sortOf t₁ >>= λ s₁ => sortOf t₂ >>= λ s₂ =>
@@ -120,8 +120,8 @@ def checkBinaryBV : OptionM Term → OptionM Term →
   | (bv m, bv n) => if (m = n) then (constr m t₁ t₂) else none
   | (_, _) => none
 
-/- Given two lists, and a function that transforms elements of
-   each list into a third type, apply the function index-wise
+/- Given two lists, and a function that transforms elements of 
+   each list into a third type, apply the function index-wise 
    on the lists -/
 def zip {α β γ : Type} : List α → List β →  (α → β → γ) → List γ
    | (h₁ :: t₁), (h₂ :: t₂), p => (p h₁ h₂) :: (zip t₁ t₂ p)
@@ -131,13 +131,13 @@ def zip {α β γ : Type} : List α → List β →  (α → β → γ) → List
 /-
 bblastBvBitwise ot₁ ot₂ const
 checks that ot₁ and ot₂ are BVs of the same length
-and returns an OptionM List of OptionM Terms that
+and returns an Option List of Option terms that
 has the bitwise application of const to the
 respective elements of ot₁ and ot₂
 -/
-def bblastBvBitwise (ot₁ ot₂ : OptionM Term)
- (constructor : OptionM Term → OptionM Term → OptionM Term) : OptionM Term :=
-    ot₁ >>= λ t₁ => ot₂ >>= λ t₂ =>
+def bblastBvBitwise (ot₁ ot₂ : Option term)
+ (constructor : Option term → Option term → Option term) : Option term :=
+    ot₁ >>= λ t₁ => ot₂ >>= λ t₂ => 
     sortOf t₁ >>= λ s₁ => sortOf t₂ >>= λ s₂ =>
       match (s₁, s₂) with
       |  (bv m, bv n) =>
@@ -151,54 +151,43 @@ def bblastBvBitwise (ot₁ ot₂ : OptionM Term)
  BV equality
 ----------- -/
 
--- If Terms are well-typed, construct their BV Eq application
-def mkBvEq : OptionM Term → OptionM Term → OptionM Term :=
+-- If terms are well-typed, construct their BV Eq application
+def mkBvEq : Option term → Option term → Option term :=
   λ ot₁ ot₂ => checkBinaryBV ot₁ ot₂ bvEq
 
 /-
-If Terms are well-typed, construct their bit-blasted BV eq
+If terms are well-typed, construct their bit-blasted BV eq
 [x₀, x₁, ... , xₙ] = [y₀, y₁, ... , yₙ]
 ---------------------------------------
        x₀ = y₀ ∧ ... ∧ xₙ = yₙ
 -/
-def bblastBvEq : OptionM Term → OptionM Term → OptionM Term :=
+def bblastBvEq : Option term → Option term → Option term :=
   λ ot₁ ot₂ =>
     ot₁ >>= λ t₁ => ot₂ >>= λ t₂ =>
-    sortOf t₁ >>= λ s₁ => sortOf t₂ >>= λ s₂ =>
+    sortOf t₁ >>= λ s₁ => sortOf t₂ >>= λ s₂ => 
     match (s₁, s₂) with
-    | (bv m, bv n) =>
+    |  (bv m, bv n) =>
       if (m = n) then (
             mkAndN (zip (bitOfN t₁ m) (bitOfN t₂ m) mkEq)
       ) else some top
     | (_, _) => some bot
-
 -- 0000 = 1111
-#check bblastBvEq (val (Value.bitvec [false, false, false, false]) (bv 4))
-  (val (Value.bitvec [true, true, true, true]) (bv 4))
-#eval OptionMTermToString (termEval (bblastBvEq (val (Value.bitvec [false, false, false, false]) (bv 4))
-  (val (Value.bitvec [true, true, true, true]) (bv 4))))
-#eval OptionMTermToString (bblastBvEq (val (Value.bitvec [false, false, false, false]) (bv 4))
-  (val (Value.bitvec [true, true, true, true]) (bv 4)))
+#eval bblastBvEq (val (value.bitvec [false, false, false, false]) (bv 4))
+  (val (value.bitvec [true, true, true, true]) (bv 4))
+#eval termEval (bblastBvEq (val (value.bitvec [false, false, false, false]) (bv 4))
+  (val (value.bitvec [true, true, true, true]) (bv 4)))
 -- 010 = 010
--- #check bblastBvEq (val (Value.bitvec [false, true, false]) (bv 3))
---   (val (Value.bitvec [false, true, false]) (bv 3))
---
--- check (bblastBvEq (val (Value.bitvec [false, true, false]) (bv 3))
---                   (val (Value.bitvec [false, true, false]) (bv 3)))
---
--- #check OptionMTermToString
---   (termEval (bblastBvEq (val (Value.bitvec [false, true, false]) (bv 3))
---   (val (Value.bitvec [false, true, false]) (bv 3))))
-
+#eval bblastBvEq (val (value.bitvec [false, true, false]) (bv 3))
+  (val (value.bitvec [false, true, false]) (bv 3))
+#eval termEval (bblastBvEq (val (value.bitvec [false, true, false]) (bv 3))
+  (val (value.bitvec [false, true, false]) (bv 3)))
 -- Using variables
-#check bblastBvEq (const (mkName "x") (bv 4))
-  (val (Value.bitvec [false, false, false, false]) (bv 4))
-#check bblastBvEq (const (mkName "x") (bv 4)) (const (mkName "y") (bv 4))
-
--- #check OptionMTermToString (bblastBvEq (const (mkName "x") (bv 4)) (const (mkName "y") (bv 4)))
+#eval bblastBvEq (const 21 (bv 4))
+  (val (value.bitvec [false, false, false, false]) (bv 4))
+#eval bblastBvEq (const 21 (bv 4)) (const 22 (bv 4))
 
 -- Bit-blasting BvEq rule
-axiom bbBvEq : ∀ {t₁ t₂ : OptionM Term},
+axiom bbBvEq : ∀ {t₁ t₂ : Option term},
   thHolds (mkEq (mkBvEq t₁ t₂) (bblastBvEq t₁ t₂))
 
 
@@ -206,29 +195,29 @@ axiom bbBvEq : ∀ {t₁ t₂ : OptionM Term},
  BV not
 ------- -/
 
--- If Term is a BV, construct its BV Not application
-def mkBvNot : OptionM Term → OptionM Term :=
+-- If term is a BV, construct its BV Not application
+def mkBvNot : Option term → Option term :=
   λ ot => ot >>= λ t => sortOf t >>= λ s =>
   match s with
   | bv n => bvNot n t
-  | _ => none
+  | _ => none 
 
 /-
-If Term is a BV, construct its bit-blasted BV not
+If term is a BV, construct its bit-blasted BV not
 ¬bv [x₀, x₁, ... , xₙ]
 ----------------------
  [¬x₀, ¬x₁, ... , ¬x]
 -/
-def bblastBvNot (ot : OptionM Term) : OptionM Term :=
+def bblastBvNot (ot : Option term) : Option term :=
   ot >>= λ t => sortOf t >>= λ s =>
     match s with
     | bv n => mkBbT (List.map mkNot (bitOfN t n))
     | _ => none
-#check bblastBvNot (val (Value.bitvec [false, false, false, false]) (bv 4))
-#check bblastBvNot (const (mkName "x") (bv 4))
+#eval bblastBvNot (val (value.bitvec [false, false, false, false]) (bv 4))
+#eval bblastBvNot (const 21 (bv 4))
 
 -- Bit-blasting BvNot rule
-axiom bbBvNot : ∀ {t : OptionM Term},
+axiom bbBvNot : ∀ {t : Option term},
   thHolds (mkEq (mkBvNot t) (bblastBvNot t))
 
 
@@ -236,27 +225,27 @@ axiom bbBvNot : ∀ {t : OptionM Term},
  BV and
 -------- -/
 
--- If Terms are well-typed, construct their BV And application
-def mkBvAnd : OptionM Term → OptionM Term → OptionM Term :=
+-- If terms are well-typed, construct their BV And application
+def mkBvAnd : Option term → Option term → Option term :=
   λ ot₁ ot₂ => checkBinaryBV ot₁ ot₂ bvAnd
 
 /-
-If Terms are well-typed, construct their bit-blasted BV and
+If terms are well-typed, construct their bit-blasted BV and
 [x₀ x₁ ... xₙ] ∧bv [y₀ y₁ ... yₙ]
 ---------------------------------
  [x₀ ∧ y₀, x₁ ∧ x₂, ... xₙ ∧ yₙ]
 -/
-def bblastBvAnd : OptionM Term → OptionM Term → OptionM Term :=
+def bblastBvAnd : Option term → Option term → Option term :=
   λ ot₁ ot₂ => bblastBvBitwise ot₁ ot₂ mkAnd
 
-#check bblastBvAnd (val (Value.bitvec [false, false, false, false]) (bv 4))
-  (val (Value.bitvec [true, true, true, true]) (bv 4))
-#check bblastBvAnd (const (mkName "x") (bv 4))
-  (val (Value.bitvec [false, false, false, false]) (bv 4))
-#check bblastBvAnd (const (mkName "x") (bv 4)) (const (mkName "y") (bv 4))
+#eval bblastBvAnd (val (value.bitvec [false, false, false, false]) (bv 4))
+  (val (value.bitvec [true, true, true, true]) (bv 4))
+#eval bblastBvAnd (const 21 (bv 4))
+  (val (value.bitvec [false, false, false, false]) (bv 4))
+#eval bblastBvAnd (const 21 (bv 4)) (const 22 (bv 4))
 
 -- Bit-blasting BvAnd rule
-axiom bbBvAnd : ∀ {t₁ t₂ : OptionM Term},
+axiom bbBvAnd : ∀ {t₁ t₂ : Option term},
   thHolds (mkEq (mkBvAnd t₁ t₂) (bblastBvAnd t₁ t₂))
 
 
@@ -264,28 +253,28 @@ axiom bbBvAnd : ∀ {t₁ t₂ : OptionM Term},
  BV or
 ----- -/
 
--- If Terms are well-typed, construct their BV Or application
-def mkBvOr : OptionM Term → OptionM Term → OptionM Term :=
+-- If terms are well-typed, construct their BV Or application
+def mkBvOr : Option term → Option term → Option term :=
   λ ot₁ ot₂ => checkBinaryBV ot₁ ot₂ bvOr
 
 /-
-If Terms are well-typed, construct their bit-blasted BV or
+If terms are well-typed, construct their bit-blasted BV or
 [x₀ x₁ ... xₙ] ∨bv [y₀ y₁ ... yₙ]
 ---------------------------------
  [x₀ ∨ y₀, x₁ ∨ x₂, ... xₙ ∨ yₙ]
 -/
-def bblastBvOr : OptionM Term → OptionM Term → OptionM Term :=
+def bblastBvOr : Option term → Option term → Option term :=
   λ ot₁ ot₂ => bblastBvBitwise ot₁ ot₂ mkOr
 
-#check bblastBvOr (val (Value.bitvec [false, false, false, false]) (bv 4))
-  (val (Value.bitvec [true, true, true, true]) (bv 4))
-#check bblastBvOr (const (mkName "x") (bv 4))
-  (val (Value.bitvec [false, false, false, false]) (bv 4))
-#check bblastBvOr (const (mkName "x") (bv 4)) (const (mkName "y") (bv 4))
-#check mkBbT (bitOfN (val (Value.bitvec [true, true, true, true]) (bv 4)) 4)
+#eval bblastBvOr (val (value.bitvec [false, false, false, false]) (bv 4))
+  (val (value.bitvec [true, true, true, true]) (bv 4))
+#eval bblastBvOr (const 21 (bv 4))
+  (val (value.bitvec [false, false, false, false]) (bv 4))
+#eval bblastBvOr (const 21 (bv 4)) (const 22 (bv 4))
+#eval mkBbT (bitOfN (val (value.bitvec [true, true, true, true]) (bv 4)) 4)
 
 -- Bit-blasting BvOr rule
-axiom bbBvOr : ∀ {t₁ t₂ : OptionM Term},
+axiom bbBvOr : ∀ {t₁ t₂ : Option term},
   thHolds (mkEq (mkBvOr t₁ t₂) (bblastBvOr t₁ t₂))
 
 
@@ -295,56 +284,56 @@ axiom bbBvOr : ∀ {t₁ t₂ : OptionM Term},
  BV unsigned less than
 --------------------- -/
 
--- If Terms are well-typed, construct their BV Ult application
-def mkBvUlt : OptionM Term → OptionM Term → OptionM Term :=
+-- If terms are well-typed, construct their BV Ult application
+def mkBvUlt : Option term → Option term → Option term :=
   λ ot₁ ot₂ => checkBinaryBV ot₁ ot₂ bvUlt
 
 /-
-[x₀, x₁, ... , xₙ] <ᵤ [y₀, y₁, ... , yₙ] =
+[x₀, x₁, ... , xₙ] <ᵤ [y₀, y₁, ... , yₙ] = 
   (¬x₀ ∧ y₀) ∨ ((x₀ ↔ y₀) ∧ ([x₁, ... , xₙ] <ᵤ [y₁, ... , yₙ]))
 -/
-def boolListUlt : List (OptionM Term) → List (OptionM Term) → OptionM Term
+def boolListUlt : List (Option term) → List (Option term) → Option term
 | [h₁], [h₂] => mkAnd (mkNot h₁) h₂
 | (h₁ :: t₁), (h₂ :: t₂) => (mkOr (mkAnd (mkNot h₁) h₂) (mkAnd (mkEq h₁ h₂) (boolListUlt t₁ t₂)))
 | _, _ => none
 
 /-
-If Terms are well-typed, construct their bit-blasted
+If terms are well-typed, construct their bit-blasted 
 unsigned less than comparison
 -/
-def bblastBvUlt : OptionM Term → OptionM Term → OptionM Term :=
+def bblastBvUlt : Option term → Option term → Option term :=
   λ ot₁ ot₂ =>
-    ot₁ >>= λ t₁ => ot₂ >>= λ t₂ =>
+    ot₁ >>= λ t₁ => ot₂ >>= λ t₂ => 
     sortOf t₁ >>= λ s₁ => sortOf t₂ >>= λ s₂ =>
     match (s₁, s₂) with
-    |  (bv m, bv n) =>
+    |  (bv m, bv n) => 
       if (m = n) then (
             boolListUlt (bitOfN t₁ m) (bitOfN t₂ m)
       ) else some top
     | (_, _) => some bot
 
 -- 0000 <ᵤ 1111
-#check bblastBvUlt (val (Value.bitvec [false, false, false, false]) (bv 4))
-  (val (Value.bitvec [true, true, true, true]) (bv 4))
-#check termEval (bblastBvUlt (val (Value.bitvec [false, false, false, false]) (bv 4))
-  (val (Value.bitvec [true, true, true, true]) (bv 4)))
+#eval bblastBvUlt (val (value.bitvec [false, false, false, false]) (bv 4))
+  (val (value.bitvec [true, true, true, true]) (bv 4))
+#eval termEval (bblastBvUlt (val (value.bitvec [false, false, false, false]) (bv 4))
+  (val (value.bitvec [true, true, true, true]) (bv 4)))
 -- 0010 <ᵤ 0011
-#check bblastBvUlt (val (Value.bitvec [false, false, true, false]) (bv 4))
-  (val (Value.bitvec [false, false, true, true]) (bv 4))
-#check termEval (bblastBvUlt (val (Value.bitvec [false, false, true, false]) (bv 4))
-  (val (Value.bitvec [false, false, true, true]) (bv 4)))
+#eval bblastBvUlt (val (value.bitvec [false, false, true, false]) (bv 4))
+  (val (value.bitvec [false, false, true, true]) (bv 4))
+#eval termEval (bblastBvUlt (val (value.bitvec [false, false, true, false]) (bv 4))
+  (val (value.bitvec [false, false, true, true]) (bv 4)))
 -- 10 <ᵤ 01
-#check bblastBvUlt (val (Value.bitvec [true, false]) (bv 2))
-  (val (Value.bitvec [false, true]) (bv 2))
-#check termEval (bblastBvUlt (val (Value.bitvec [true, false]) (bv 2))
-  (val (Value.bitvec [false, true]) (bv 2)))
+#eval bblastBvUlt (val (value.bitvec [true, false]) (bv 2))
+  (val (value.bitvec [false, true]) (bv 2))
+#eval termEval (bblastBvUlt (val (value.bitvec [true, false]) (bv 2))
+  (val (value.bitvec [false, true]) (bv 2)))
 -- Using variables
-#check bblastBvUlt (const (mkName "x") (bv 4))
-  (val (Value.bitvec [false, false, false, false]) (bv 4))
-#check bblastBvUlt (const (mkName "x") (bv 4)) (const (mkName "y") (bv 4))
+#eval bblastBvUlt (const 21 (bv 4)) 
+  (val (value.bitvec [false, false, false, false]) (bv 4))
+#eval bblastBvUlt (const 21 (bv 4)) (const 22 (bv 4))
 
 -- Bit-blasting BvUlt rule
-axiom bbBvUlt : ∀ {t₁ t₂ : OptionM Term},
+axiom bbBvUlt : ∀ {t₁ t₂ : Option term},
   thHolds (mkEq (mkBvUlt t₁ t₂) (bblastBvUlt t₁ t₂))
 
 
@@ -352,56 +341,56 @@ axiom bbBvUlt : ∀ {t₁ t₂ : OptionM Term},
  BV unsigned greater than
 ----------------------- -/
 
--- If Terms are well-typed, construct their BV Ugt application
-def mkBvUgt : OptionM Term → OptionM Term → OptionM Term :=
+-- If terms are well-typed, construct their BV Ugt application
+def mkBvUgt : Option term → Option term → Option term :=
   λ ot₁ ot₂ => checkBinaryBV ot₁ ot₂ bvUgt
 
 /-
-[x₀, x₁, ... , xₙ] >ᵤ [y₀, y₁, ... , yₙ] =
+[x₀, x₁, ... , xₙ] >ᵤ [y₀, y₁, ... , yₙ] = 
   (x₀ ∧ ¬y₀) ∨ ((x₀ ↔ y₀) ∧ ([x₁, ... , xₙ] >ᵤ [y₁, ... , yₙ]))
 -/
-def boolListUgt : List (OptionM Term) → List (OptionM Term) → OptionM Term
+def boolListUgt : List (Option term) → List (Option term) → Option term
 | [h₁], [h₂] => mkAnd h₁ (mkNot h₂)
 | (h₁ :: t₁), (h₂ :: t₂) => (mkOr (mkAnd h₁ (mkNot h₂)) (mkAnd (mkEq h₁ h₂) (boolListUgt t₁ t₂)))
 | _, _ => none
 
 /-
-If Terms are well-typed, construct their bit-blasted
+If terms are well-typed, construct their bit-blasted 
 unsigned greater than comparison
 -/
-def bblastBvUgt : OptionM Term → OptionM Term → OptionM Term :=
+def bblastBvUgt : Option term → Option term → Option term :=
   λ ot₁ ot₂ =>
-    ot₁ >>= λ t₁ => ot₂ >>= λ t₂ =>
+    ot₁ >>= λ t₁ => ot₂ >>= λ t₂ => 
     sortOf t₁ >>= λ s₁ => sortOf t₂ >>= λ s₂ =>
     match (s₁, s₂) with
-    |  (bv m, bv n) =>
+    |  (bv m, bv n) => 
       if (m = n) then (
             boolListUgt (bitOfN t₁ m) (bitOfN t₂ m)
       ) else some top
     | (_, _) => some bot
 
 -- 1111 >ᵤ 0000
-#check bblastBvUgt (val (Value.bitvec [true, true, true, true]) (bv 4))
-  (val (Value.bitvec [false, false, false, false]) (bv 4))
-#check termEval (bblastBvUgt (val (Value.bitvec [true, true, true, true]) (bv 4))
-  (val (Value.bitvec [false, false, false, false]) (bv 4)))
+#eval bblastBvUgt (val (value.bitvec [true, true, true, true]) (bv 4))
+  (val (value.bitvec [false, false, false, false]) (bv 4))
+#eval termEval (bblastBvUgt (val (value.bitvec [true, true, true, true]) (bv 4))
+  (val (value.bitvec [false, false, false, false]) (bv 4)))
 -- 0011 >ᵤ 0010
-#check bblastBvUgt (val (Value.bitvec [false, false, true, true]) (bv 4))
-  (val (Value.bitvec [false, false, true, false]) (bv 4))
-#check termEval (bblastBvUgt (val (Value.bitvec [false, false, true, true]) (bv 4))
-  (val (Value.bitvec [false, false, true, false]) (bv 4)))
+#eval bblastBvUgt (val (value.bitvec [false, false, true, true]) (bv 4))
+  (val (value.bitvec [false, false, true, false]) (bv 4))
+#eval termEval (bblastBvUgt (val (value.bitvec [false, false, true, true]) (bv 4))
+  (val (value.bitvec [false, false, true, false]) (bv 4)))
 -- 01 >ᵤ 10
-#check bblastBvUgt (val (Value.bitvec [false, true]) (bv 2))
-  (val (Value.bitvec [true, false]) (bv 2))
-#check termEval (bblastBvUgt (val (Value.bitvec [false, true]) (bv 2))
-  (val (Value.bitvec [true, false]) (bv 2)))
+#eval bblastBvUgt (val (value.bitvec [false, true]) (bv 2))
+  (val (value.bitvec [true, false]) (bv 2))
+#eval termEval (bblastBvUgt (val (value.bitvec [false, true]) (bv 2))
+  (val (value.bitvec [true, false]) (bv 2)))
 -- Using variables
-#check bblastBvUgt (const (mkName "x") (bv 4))
-  (val (Value.bitvec [false, false, false, false]) (bv 4))
-#check bblastBvUgt (const (mkName "x") (bv 4)) (const (mkName "y") (bv 4))
+#eval bblastBvUgt (const 21 (bv 4)) 
+  (val (value.bitvec [false, false, false, false]) (bv 4))
+#eval bblastBvUgt (const 21 (bv 4)) (const 22 (bv 4))
 
 -- Bit-blasting BvUgt rule
-axiom bbBvUgt : ∀ {t₁ t₂ : OptionM Term},
+axiom bbBvUgt : ∀ {t₁ t₂ : Option term},
   thHolds (mkEq (mkBvUgt t₁ t₂) (bblastBvUgt t₁ t₂))
 
 
@@ -409,56 +398,56 @@ axiom bbBvUgt : ∀ {t₁ t₂ : OptionM Term},
  BV signed less than
 ------------------- -/
 
--- If Terms are well-typed, construct their BV Slt application
-def mkBvSlt : OptionM Term → OptionM Term → OptionM Term :=
+-- If terms are well-typed, construct their BV Slt application
+def mkBvSlt : Option term → Option term → Option term :=
   λ ot₁ ot₂ => checkBinaryBV ot₁ ot₂ bvSlt
 
 /-
-[x₀, x₁, ... , xₙ] <ₛ [y₀, y₁, ... , yₙ] =
+[x₀, x₁, ... , xₙ] <ₛ [y₀, y₁, ... , yₙ] = 
   (x₀ ∧ ¬y₀) ∨ (x₀ = y₀ ∧ ([x₁, ..., xₙ] <ᵤ [y₁, ..., yₙ]))
 -/
-def boolListSlt : List (OptionM Term) → List (OptionM Term) → OptionM Term
+def boolListSlt : List (Option term) → List (Option term) → Option term
 | [h₁], [h₂] => (mkAnd h₁ (mkNot h₂))
 | (h₁ :: t₁), (h₂ :: t₂) => (mkOr (mkAnd h₁ (mkNot h₂)) (mkAnd (mkEq h₁ h₂) (boolListUlt t₁ t₂)))
 | _, _ => none
 
 /-
-If Terms are well-typed, construct their bit-blasted
+If terms are well-typed, construct their bit-blasted 
 signed less than comparison
 -/
-def bblastBvSlt : OptionM Term → OptionM Term → OptionM Term :=
+def bblastBvSlt : Option term → Option term → Option term :=
   λ ot₁ ot₂ =>
-    ot₁ >>= λ t₁ => ot₂ >>= λ t₂ =>
+    ot₁ >>= λ t₁ => ot₂ >>= λ t₂ => 
     sortOf t₁ >>= λ s₁ => sortOf t₂ >>= λ s₂ =>
     match (s₁, s₂) with
-    |  (bv m, bv n) =>
+    |  (bv m, bv n) => 
       if (m = n) then (
             boolListSlt (bitOfN t₁ m) (bitOfN t₂ m)
       ) else some top
     | (_, _) => some bot
 
 -- 1111 <ₛ 0000
-#check bblastBvSlt (val (Value.bitvec [true, true, true, true]) (bv 4))
-  (val (Value.bitvec [false, false, false, false]) (bv 4))
-#check termEval (bblastBvSlt (val (Value.bitvec [true, true, true, true]) (bv 4))
-  (val (Value.bitvec [false, false, false, false]) (bv 4)))
+#eval bblastBvSlt (val (value.bitvec [true, true, true, true]) (bv 4))
+  (val (value.bitvec [false, false, false, false]) (bv 4))
+#eval termEval (bblastBvSlt (val (value.bitvec [true, true, true, true]) (bv 4))
+  (val (value.bitvec [false, false, false, false]) (bv 4)))
 -- 1010 <ₛ 1011
-#check bblastBvSlt (val (Value.bitvec [true, false, true, false]) (bv 4))
-  (val (Value.bitvec [true, false, true, true]) (bv 4))
-#check termEval (bblastBvSlt (val (Value.bitvec [true, false, true, false]) (bv 4))
-  (val (Value.bitvec [true, false, true, true]) (bv 4)))
+#eval bblastBvSlt (val (value.bitvec [true, false, true, false]) (bv 4))
+  (val (value.bitvec [true, false, true, true]) (bv 4))
+#eval termEval (bblastBvSlt (val (value.bitvec [true, false, true, false]) (bv 4))
+  (val (value.bitvec [true, false, true, true]) (bv 4)))
 -- 01 <ₛ 10
-#check bblastBvSlt (val (Value.bitvec [false, true]) (bv 2))
-  (val (Value.bitvec [true, false]) (bv 2))
-#check termEval (bblastBvSlt (val (Value.bitvec [false, true]) (bv 2))
-  (val (Value.bitvec [true, false]) (bv 2)))
+#eval bblastBvSlt (val (value.bitvec [false, true]) (bv 2))
+  (val (value.bitvec [true, false]) (bv 2))
+#eval termEval (bblastBvSlt (val (value.bitvec [false, true]) (bv 2))
+  (val (value.bitvec [true, false]) (bv 2)))
 -- Using variables
-#check bblastBvSlt (const (mkName "x") (bv 4))
-  (val (Value.bitvec [false, false, false, false]) (bv 4))
-#check bblastBvSlt (const (mkName "x") (bv 4)) (const (mkName "y") (bv 4))
+#eval bblastBvSlt (const 21 (bv 4))
+  (val (value.bitvec [false, false, false, false]) (bv 4))
+#eval bblastBvSlt (const 21 (bv 4)) (const 22 (bv 4))
 
 -- Bit-blasting BvUgt rule
-axiom bbBvSlt : ∀ {t₁ t₂ : OptionM Term},
+axiom bbBvSlt : ∀ {t₁ t₂ : Option term},
   thHolds (mkEq (mkBvSlt t₁ t₂) (bblastBvSlt t₁ t₂))
 
 
@@ -466,56 +455,56 @@ axiom bbBvSlt : ∀ {t₁ t₂ : OptionM Term},
  BV signed greater than
 ----------------------- -/
 
--- If Terms are well-typed, construct their BV Sgt application
-def mkBvSgt : OptionM Term → OptionM Term → OptionM Term :=
+-- If terms are well-typed, construct their BV Sgt application
+def mkBvSgt : Option term → Option term → Option term :=
   λ ot₁ ot₂ => checkBinaryBV ot₁ ot₂ bvSgt
 
 /-
-[x₀, x₁, ... , xₙ] >ₛ [y₀, y₁, ... , yₙ] =
+[x₀, x₁, ... , xₙ] >ₛ [y₀, y₁, ... , yₙ] = 
   (¬x₀ ∧ y₀) ∨ (x₀ = y₀ ∧ ([x₁, ..., xₙ] >ᵤ [y₁, ..., yₙ]))
 -/
-def boolListSgt : List (OptionM Term) → List (OptionM Term) → OptionM Term
+def boolListSgt : List (Option term) → List (Option term) → Option term
 | [h₁], [h₂] => (mkAnd (mkNot h₁) h₂)
 | (h₁ :: t₁), (h₂ :: t₂) => (mkOr (mkAnd (mkNot h₁) h₂) (mkAnd (mkEq h₁ h₂) (boolListUgt t₁ t₂)))
 | _, _ => none
 
 /-
-If Terms are well-typed, construct their bit-blasted
+If terms are well-typed, construct their bit-blasted 
 signed greater than comparison
 -/
-def bblastBvSgt : OptionM Term → OptionM Term → OptionM Term :=
+def bblastBvSgt : Option term → Option term → Option term :=
   λ ot₁ ot₂ =>
-    ot₁ >>= λ t₁ => ot₂ >>= λ t₂ =>
+    ot₁ >>= λ t₁ => ot₂ >>= λ t₂ => 
     sortOf t₁ >>= λ s₁ => sortOf t₂ >>= λ s₂ =>
     match (s₁, s₂) with
-    |  (bv m, bv n) =>
+    |  (bv m, bv n) => 
       if (m = n) then (
             boolListSgt (bitOfN t₁ m) (bitOfN t₂ m)
       ) else some top
     | (_, _) => some bot
 
 -- 0000 >ₛ 1111
-#check bblastBvSgt (val (Value.bitvec [false, false, false, false]) (bv 4))
-  (val (Value.bitvec [true, true, true, true]) (bv 4))
-#check termEval (bblastBvSgt (val (Value.bitvec [false, false, false, false]) (bv 4))
-  (val (Value.bitvec [true, true, true, true]) (bv 4)))
+#eval bblastBvSgt (val (value.bitvec [false, false, false, false]) (bv 4))
+  (val (value.bitvec [true, true, true, true]) (bv 4))
+#eval termEval (bblastBvSgt (val (value.bitvec [false, false, false, false]) (bv 4))
+  (val (value.bitvec [true, true, true, true]) (bv 4)))
 -- 1011 >ₛ 1010
-#check bblastBvSgt (val (Value.bitvec [true, false, true, true]) (bv 4))
-  (val (Value.bitvec [true, false, true, false]) (bv 4))
-#check termEval (bblastBvSgt (val (Value.bitvec [true, false, true, true]) (bv 4))
-  (val (Value.bitvec [true, false, true, false]) (bv 4)))
+#eval bblastBvSgt (val (value.bitvec [true, false, true, true]) (bv 4))
+  (val (value.bitvec [true, false, true, false]) (bv 4))
+#eval termEval (bblastBvSgt (val (value.bitvec [true, false, true, true]) (bv 4))
+  (val (value.bitvec [true, false, true, false]) (bv 4)))
 -- 10 >ₛ 01
-#check bblastBvSgt (val (Value.bitvec [true, false]) (bv 2))
-  (val (Value.bitvec [false, true]) (bv 2))
-#check termEval (bblastBvSgt (val (Value.bitvec [true, false]) (bv 2))
-  (val (Value.bitvec [false, true]) (bv 2)))
+#eval bblastBvSgt (val (value.bitvec [true, false]) (bv 2))
+  (val (value.bitvec [false, true]) (bv 2))
+#eval termEval (bblastBvSgt (val (value.bitvec [true, false]) (bv 2))
+  (val (value.bitvec [false, true]) (bv 2)))
 -- Using variables
-#check bblastBvSgt (const (mkName "x") (bv 4))
-  (val (Value.bitvec [false, false, false, false]) (bv 4))
-#check bblastBvSgt (const (mkName "x") (bv 4)) (const (mkName "y") (bv 4))
+#eval bblastBvSgt (const 21 (bv 4))
+  (val (value.bitvec [false, false, false, false]) (bv 4))
+#eval bblastBvSgt (const 21 (bv 4)) (const 22 (bv 4))
 
 -- Bit-blasting BvSgt rule
-axiom bbBvSgt : ∀ {t₁ t₂ : OptionM Term},
+axiom bbBvSgt : ∀ {t₁ t₂ : Option term},
   thHolds (mkEq (mkBvSgt t₁ t₂) (bblastBvSgt t₁ t₂))
 
 
@@ -525,8 +514,8 @@ axiom bbBvSgt : ∀ {t₁ t₂ : OptionM Term},
  BV addition
 ----------- -/
 
--- If Terms are well-typed, construct their BV plus application
-def mkBvAdd : OptionM Term → OptionM Term → OptionM Term :=
+-- If terms are well-typed, construct their BV plus application
+def mkBvAdd : Option term → Option term → Option term :=
   λ ot₁ ot₂ => checkBinaryBV ot₁ ot₂ bvAdd
 
 /-
@@ -538,58 +527,58 @@ where car₀ = ⊥
       car_{i+1} = (xᵢ ∧ yᵢ) ∨ ((xᵢ ⊕ yᵢ) ∧ carᵢ)
 Then reverse again
 -/
-def bitAdder : OptionM Term → OptionM Term → OptionM Term → OptionM Term × OptionM Term
-| x, y, carry => (mkXor (mkXor x y) carry,
+def bitAdder : Option term → Option term → Option term → Option term × Option term
+| x, y, carry => (mkXor (mkXor x y) carry, 
   mkOr (mkAnd x y) (mkAnd (mkXor x y) carry))
-#check (bitAdder top top top)
-#check termEval (bitAdder top top top).1
-#check termEval (bitAdder top top top).2
-def boolListAddAux : OptionM Term → List (OptionM Term) → List (OptionM Term) → List (OptionM Term)
+#eval (bitAdder top top top)
+#eval termEval (bitAdder top top top).1
+#eval termEval (bitAdder top top top).2
+def boolListAddAux : Option term → List (Option term) → List (Option term) → List (Option term)
 | c, (h₁ :: t₁), (h₂ :: t₂) => (bitAdder h₁ h₂ c).1 :: (boolListAddAux (bitAdder h₁ h₂ c).2 t₁ t₂)
 | c, [], [] => []
 | _, _, _ => []
-def boolListAdd : List (OptionM Term) → List (OptionM Term) → OptionM Term
+def boolListAdd : List (Option term) → List (Option term) → Option term
 | l₁, l₂ => mkBbT (List.reverse (boolListAddAux bot l₁ l₂))
 
--- If Terms are well-typed, construct their bit-blasted BV add
-def bblastBvAdd : OptionM Term → OptionM Term → OptionM Term :=
-  λ ot₁ ot₂ =>
-  ot₁ >>= λ t₁ => ot₂ >>= λ t₂ =>
+-- If terms are well-typed, construct their bit-blasted BV add
+def bblastBvAdd : Option term → Option term → Option term :=
+  λ ot₁ ot₂ => 
+  ot₁ >>= λ t₁ => ot₂ >>= λ t₂ => 
     sortOf t₁ >>= λ s₁ => sortOf t₂ >>= λ s₂ =>
     match (s₁, s₂) with
-    |  (bv m, bv n) =>
+    |  (bv m, bv n) => 
       if (m = n) then (
             boolListAdd (bitOfNRev t₁ m) (bitOfNRev t₂ m)
       ) else some top
     | (_, _) => some bot
 
 -- 0000 + 1111
-#check bblastBvAdd (val (Value.bitvec [false, false, false, false]) (bv 4))
-  (val (Value.bitvec [true, true, true, true]) (bv 4))
-#check termEval (bblastBvAdd (val (Value.bitvec [false, false, false, false]) (bv 4))
-  (val (Value.bitvec [true, true, true, true]) (bv 4)))
+#eval bblastBvAdd (val (value.bitvec [false, false, false, false]) (bv 4))
+  (val (value.bitvec [true, true, true, true]) (bv 4))
+#eval termEval (bblastBvAdd (val (value.bitvec [false, false, false, false]) (bv 4))
+  (val (value.bitvec [true, true, true, true]) (bv 4)))
 -- 1111 + 1111
-#check bblastBvAdd (val (Value.bitvec [true, true, true, true]) (bv 4))
-  (val (Value.bitvec [true, true, true, true]) (bv 4))
-#check termEval (bblastBvAdd (val (Value.bitvec [true, true, true, true]) (bv 4))
-  (val (Value.bitvec [true, true, true, true]) (bv 4)))
+#eval bblastBvAdd (val (value.bitvec [true, true, true, true]) (bv 4))
+  (val (value.bitvec [true, true, true, true]) (bv 4))
+#eval termEval (bblastBvAdd (val (value.bitvec [true, true, true, true]) (bv 4))
+  (val (value.bitvec [true, true, true, true]) (bv 4)))
 -- 0101 + 1010
-#check bblastBvAdd (val (Value.bitvec [false, true, false, true]) (bv 4))
-  (val (Value.bitvec [true, false, true, false]) (bv 4))
-#check termEval (bblastBvAdd (val (Value.bitvec [false, true, false, true]) (bv 4))
-  (val (Value.bitvec [true, false, true, false]) (bv 4)))
+#eval bblastBvAdd (val (value.bitvec [false, true, false, true]) (bv 4))
+  (val (value.bitvec [true, false, true, false]) (bv 4))
+#eval termEval (bblastBvAdd (val (value.bitvec [false, true, false, true]) (bv 4))
+  (val (value.bitvec [true, false, true, false]) (bv 4)))
 -- 1111 + 0001
-#check bblastBvAdd (val (Value.bitvec [true, true, true, true]) (bv 4))
-  (val (Value.bitvec [false, false, false, true]) (bv 4))
-#check termEval (bblastBvAdd (val (Value.bitvec [true, true, true, true]) (bv 4))
-  (val (Value.bitvec [false, false, false, true]) (bv 4)))
+#eval bblastBvAdd (val (value.bitvec [true, true, true, true]) (bv 4))
+  (val (value.bitvec [false, false, false, true]) (bv 4))
+#eval termEval (bblastBvAdd (val (value.bitvec [true, true, true, true]) (bv 4))
+  (val (value.bitvec [false, false, false, true]) (bv 4)))
 -- Using variables
-#check bblastBvAdd (const (mkName "x") (bv 4))
-  (val (Value.bitvec [false, false, false, false]) (bv 4))
-#check bblastBvAdd (const (mkName "x") (bv 4)) (const (mkName "y") (bv 4))
+#eval bblastBvAdd (const 21 (bv 4))
+  (val (value.bitvec [false, false, false, false]) (bv 4))
+#eval bblastBvAdd (const 21 (bv 4)) (const 22 (bv 4))
 
 -- Bit-blasting BvAdd rule
-axiom bbBvAdd : ∀ {t₁ t₂ : OptionM Term},
+axiom bbBvAdd : ∀ {t₁ t₂ : Option term},
   thHolds (mkEq (mkBvAdd t₁ t₂) (bblastBvAdd t₁ t₂))
 
 
@@ -597,50 +586,50 @@ axiom bbBvAdd : ∀ {t₁ t₂ : OptionM Term},
  BV Negation
 ------------ -/
 
--- If Term is a BV, construct its BV Neg application
-def mkBvNeg : OptionM Term → OptionM Term :=
+-- If term is a BV, construct its BV Neg application
+def mkBvNeg : Option term → Option term :=
   λ ot => ot >>= λ t => sortOf t >>= λ s =>
   match s with
   | bv n => bvNot n t
-  | _ => none
+  | _ => none 
 
-/- genRevOne n generates the list
+/- genRevOne n generates the list 
    [(some top) (some bot) ... (some bot)]
    where there are n-1 (some bot) elements -/
-def genZeros : Nat → List (OptionM Term)
+def genZeros : Nat → List (Option term)
 | 0 => []
 | n + 1 => (some bot) :: genZeros n
-def genRevOne : Nat → List (OptionM Term) :=
+def genRevOne : Nat → List (Option term) :=
   λ n => (some top) :: genZeros (n - 1)
-#check genZeros 3
-#check genRevOne 4
+#eval genZeros 3
+#eval genRevOne 4
 
 /-
-If Term is well-typed, construct its bit-blasted BV neg
+If term is well-typed, construct its bit-blasted BV neg
 -bv x = ((¬bv x) +bv 1)
           OR
 bvneg x = bvadd (bvnot x) 1
 -/
-def bblastBvNeg : OptionM Term → OptionM Term :=
-  λ ot =>
-  ot >>= λ t => sortOf t >>= λ s =>
+def bblastBvNeg : Option term → Option term :=
+  λ ot => 
+  ot >>= λ t => sortOf t >>= λ s => 
     match s with
     |  bv m => boolListAdd (List.map mkNot (bitOfNRev t m)) (genRevOne m)
     | _ => some bot
 -- -0000
-#check bblastBvNeg (val (Value.bitvec [false, false, false, false]) (bv 4))
-#check termEval (bblastBvNeg (val (Value.bitvec [false, false, false, false]) (bv 4)))
+#eval bblastBvNeg (val (value.bitvec [false, false, false, false]) (bv 4))
+#eval termEval (bblastBvNeg (val (value.bitvec [false, false, false, false]) (bv 4)))
 -- -0001
-#check bblastBvNeg (val (Value.bitvec [false, false, false, true]) (bv 4))
-#check termEval (bblastBvNeg (val (Value.bitvec [false, false, false, true]) (bv 4)))
+#eval bblastBvNeg (val (value.bitvec [false, false, false, true]) (bv 4))
+#eval termEval (bblastBvNeg (val (value.bitvec [false, false, false, true]) (bv 4)))
 -- -1111
-#check bblastBvNeg (val (Value.bitvec [true, true, true, true]) (bv 4))
-#check termEval (bblastBvNeg (val (Value.bitvec [true, true, true, true]) (bv 4)))
+#eval bblastBvNeg (val (value.bitvec [true, true, true, true]) (bv 4))
+#eval termEval (bblastBvNeg (val (value.bitvec [true, true, true, true]) (bv 4)))
 -- Using variables
-#check bblastBvNeg (const (mkName "x") (bv 4))
+#eval bblastBvNeg (const 21 (bv 4))
 
 -- Bit-blasting BvNeg rule
-axiom bbBvNeg : ∀ {t : OptionM Term},
+axiom bbBvNeg : ∀ {t : Option term},
   thHolds (mkEq (mkBvNeg t) (bblastBvNeg t))
 
 
@@ -650,16 +639,16 @@ axiom bbBvNeg : ∀ {t : OptionM Term},
  BV Extraction
 ------------ -/
 
--- If Terms are well-typed, construct their BV Extraction application
-def mkBvExtract : OptionM Term → OptionM Term → OptionM Term → OptionM Term :=
-  λ ot oi oj =>
+-- If terms are well-typed, construct their BV Extraction application
+def mkBvExtract : Option term → Option term → Option term → Option term :=
+  λ ot oi oj => 
     ot >>= λ t => sortOf t >>= λ s =>
     oi >>= λ i => sortOf i >>= λ si =>
     oj >>= λ j => sortOf i >>= λ sj =>
   match s, si, sj with
   | bv n, intSort, intSort =>
     match i, j with
-    | (val (Value.integer i₁) intSort), (val (Value.integer j₁) intSort) =>
+    | (val (value.integer i₁) intSort), (val (value.integer j₁) intSort) =>
       if (0 ≤ j₁ ∧ j₁ ≤ i₁ ∧ i₁ < n) then
         (bvExtract n (Int.toNat i₁) (Int.toNat j₁) t i j)
       else
@@ -672,41 +661,41 @@ def removeLastN : List α → Nat → List α
 | l, n+1 => removeLastN (List.dropLast l) n
 
 /-
-If Terms are well-typed, construct their bit-blasted BV extraction
+If terms are well-typed, construct their bit-blasted BV extraction
 [x₀ ... xₙ]   0 ≤ j ≤ i < n
 ----------------------------
        [xⱼ ... xᵢ]
 -/
-def bblastBvExtract : OptionM Term → OptionM Term → OptionM Term → OptionM Term :=
-  λ ot oi oj =>
+def bblastBvExtract : Option term → Option term → Option term → Option term :=
+  λ ot oi oj => 
     ot >>= λ t => sortOf t >>= λ s =>
     oi >>= λ i => sortOf i >>= λ si =>
     oj >>= λ j => sortOf i >>= λ sj =>
   match s, si, sj with
   | bv n, intSort, intSort =>
     match i, j with
-    | (val (Value.integer i₁) intSort), (val (Value.integer j₁) intSort) =>
-      if (0 ≤ j₁ ∧ j₁ ≤ i₁ ∧ i₁ < n) then
+    | (val (value.integer i₁) intSort), (val (value.integer j₁) intSort) =>
+      if (0 ≤ j₁ ∧ j₁ ≤ i₁ ∧ i₁ < n) then 
          mkBbT (removeLastN (List.drop (n - (Int.toNat i₁) - 1) (bitOfN t n)) (Int.toNat j₁))
       else
         none
     | _, _ => none
   | _, _, _ => none
-#check bblastBvExtract (val (Value.bitvec [false, false, true, false]) (bv 4))
-  (val (Value.integer 3) intSort) (val (Value.integer 2) intSort)
-#check bblastBvExtract (val (Value.bitvec [false, false, true, false]) (bv 4))
-  (val (Value.integer 1) intSort) (val (Value.integer 1) intSort)
-#check bblastBvExtract (val (Value.bitvec [false, false, true, false]) (bv 4))
-  (val (Value.integer 3) intSort) (val (Value.integer 0) intSort)
+#eval bblastBvExtract (val (value.bitvec [false, false, true, false]) (bv 4))
+  (val (value.integer 3) intSort) (val (value.integer 2) intSort)
+#eval bblastBvExtract (val (value.bitvec [false, false, true, false]) (bv 4))
+  (val (value.integer 1) intSort) (val (value.integer 1) intSort)
+#eval bblastBvExtract (val (value.bitvec [false, false, true, false]) (bv 4))
+  (val (value.integer 3) intSort) (val (value.integer 0) intSort)
 -- Bad call
-#check bblastBvExtract (val (Value.bitvec [false, false, true, false]) (bv 4))
-  (val (Value.integer 1) intSort) (val (Value.integer 2) intSort)
+#eval bblastBvExtract (val (value.bitvec [false, false, true, false]) (bv 4))
+  (val (value.integer 1) intSort) (val (value.integer 2) intSort)
 -- Using variables
-#check bblastBvExtract (const (mkName "x") (bv 4)) (val (Value.integer 2) intSort)
-  (val (Value.integer 1) intSort)
+#eval bblastBvExtract (const 21 (bv 4)) (val (value.integer 2) intSort) 
+  (val (value.integer 1) intSort)
 
 -- Bit-blasting BvExtract rule
-axiom bbBvExtract : ∀ {t₁ t₂ t₃ : OptionM Term},
+axiom bbBvExtract : ∀ {t₁ t₂ t₃ : Option term},
   thHolds (mkEq (mkBvExtract t₁ t₂ t₃) (bblastBvExtract t₁ t₂ t₃))
 
 
@@ -714,8 +703,8 @@ axiom bbBvExtract : ∀ {t₁ t₂ t₃ : OptionM Term},
  BV Concatenation
 ---------------- -/
 
--- If Terms are well-typed, construct their BV concat application
-def mkBvConcat : OptionM Term → OptionM Term → OptionM Term :=
+-- If terms are well-typed, construct their BV concat application
+def mkBvConcat : Option term → Option term → Option term :=
   λ ot₁ ot₂ => ot₁ >>= λ t₁ => sortOf t₁ >>= λ s₁ =>
                ot₂ >>= λ t₂ => sortOf t₂ >>= λ s₂ =>
   match s₁, s₂ with
@@ -723,33 +712,33 @@ def mkBvConcat : OptionM Term → OptionM Term → OptionM Term :=
   | _, _ => none
 
 /-
-If Terms are BVs construct their bit-blasted BV concat
+If terms are BVs construct their bit-blasted BV concat
 [x₀ x₁ ... xₙ] ++ [y₀ y₁ ... yₙ]
 ---------------------------------
    [y₀ y₁ ... yₙ x₀ x₁ ... xₙ]
 -/
-def bblastBvConcat : OptionM Term → OptionM Term → OptionM Term :=
-  λ ot₁ ot₂ => ot₁ >>= λ t₁ => sortOf t₁ >>= λ s₁ =>
-               ot₂ >>= λ t₂ => sortOf t₂ >>= λ s₂ =>
+def bblastBvConcat : Option term → Option term → Option term :=
+  λ ot₁ ot₂ => ot₁ >>= λ t₁ => sortOf t₁ >>= λ s₁ => 
+               ot₂ >>= λ t₂ => sortOf t₂ >>= λ s₂ => 
     match s₁, s₂ with
     | bv m, bv n => mkBbT (List.append (bitOfN t₂ n) (bitOfN t₁ m))
     | _, _ => none
 -- 0000 ++ 1111
-#check bblastBvConcat (val (Value.bitvec [false, false, false, false]) (bv 4))
-  (val (Value.bitvec [true, true, true, true]) (bv 4))
+#eval bblastBvConcat (val (value.bitvec [false, false, false, false]) (bv 4))
+  (val (value.bitvec [true, true, true, true]) (bv 4))
 -- 11 + 111
-#check bblastBvConcat (val (Value.bitvec [true, true]) (bv 2))
-  (val (Value.bitvec [true, true, true]) (bv 3))
+#eval bblastBvConcat (val (value.bitvec [true, true]) (bv 2))
+  (val (value.bitvec [true, true, true]) (bv 3))
 -- 1 + 110
-#check bblastBvConcat (val (Value.bitvec [true]) (bv 1))
-  (val (Value.bitvec [true, true, false]) (bv 3))
+#eval bblastBvConcat (val (value.bitvec [true]) (bv 1))
+  (val (value.bitvec [true, true, false]) (bv 3))
 -- Using variables
-#check bblastBvConcat (const (mkName "x") (bv 2))
-  (val (Value.bitvec [false, false]) (bv 2))
-#check bblastBvConcat (const (mkName "x") (bv 2)) (const (mkName "y") (bv 2))
+#eval bblastBvConcat (const 21 (bv 2))
+  (val (value.bitvec [false, false]) (bv 2))
+#eval bblastBvConcat (const 21 (bv 2)) (const 22 (bv 2))
 
 -- Bit-blasting BvConcat rule
-axiom bbBvConcat : ∀ {t₁ t₂ : OptionM Term},
+axiom bbBvConcat : ∀ {t₁ t₂ : Option term},
   thHolds (mkEq (mkBvConcat t₁ t₂) (bblastBvAdd t₁ t₂))
 
 
@@ -757,42 +746,42 @@ axiom bbBvConcat : ∀ {t₁ t₂ : OptionM Term},
  BV Zero Extend
 ---------------- -/
 
--- If Terms are well-typed, construct their BV zero extend application
-def mkBvZeroExt : OptionM Term → OptionM Term → OptionM Term :=
+-- If terms are well-typed, construct their BV zero extend application
+def mkBvZeroExt : Option term → Option term → Option term :=
   λ ot oi => ot >>= λ t => sortOf t >>= λ s =>
              oi >>= λ i => sortOf i >>= λ si =>
   match s, si with
-  | bv n, intSort =>
+  | bv n, intSort => 
     match i with
-    | val (Value.integer i₁) intSort => bvZeroExt n (Int.toNat i₁) t i
+    | val (value.integer i₁) intSort => bvZeroExt n (Int.toNat i₁) t i
     | _ => none
   | _, _ => none
 
 /-
-If Terms are well-typed, construct their bit-blasted BV zero extend
+If terms are well-typed, construct their bit-blasted BV zero extend
      [x₀ x₁ ... xₙ]    i
 -----------------------------
   [0₁ ... 0ᵢ x₀ x₁ ... xₙ]
 -/
-def bblastZeroExt : OptionM Term → OptionM Term → OptionM Term :=
+def bblastZeroExt : Option term → Option term → Option term :=
   λ ot oi => ot >>= λ t => sortOf t >>= λ s =>
              oi >>= λ i => sortOf i >>= λ si =>
   match s, si with
-  | bv n, intSort =>
+  | bv n, intSort => 
     match i with
-    | val (Value.integer i₁) intSort =>
+    | val (value.integer i₁) intSort => 
       mkBbT (List.append (List.replicate (Int.toNat i₁) (some bot)) (bitOfN t n))
     | _ => none
   | _, _ => none
-#check bblastZeroExt (val (Value.bitvec [true, true, true, true]) (bv 4))
-  (val (Value.integer 2) intSort)
-#check bblastZeroExt (val (Value.bitvec [true, false]) (bv 2))
-  (val (Value.integer 0) intSort)
+#eval bblastZeroExt (val (value.bitvec [true, true, true, true]) (bv 4))
+  (val (value.integer 2) intSort)
+#eval bblastZeroExt (val (value.bitvec [true, false]) (bv 2))
+  (val (value.integer 0) intSort)
 -- Using variables
-#check bblastZeroExt (const (mkName "x") (bv 4))  (val (Value.integer 2) intSort)
+#eval bblastZeroExt (const 21 (bv 4))  (val (value.integer 2) intSort)
 
 -- Bit-blasting BvZeroExt rule
-axiom bbBvZeroExt : ∀ {t₁ t₂ : OptionM Term},
+axiom bbBvZeroExt : ∀ {t₁ t₂ : Option term},
   thHolds (mkEq (mkBvZeroExt t₁ t₂) (bblastZeroExt t₁ t₂))
 
 
@@ -800,53 +789,54 @@ axiom bbBvZeroExt : ∀ {t₁ t₂ : OptionM Term},
  BV Sign Extend
 ---------------- -/
 
--- If Terms are well-typed, construct their BV sign extend application
-def mkBvSignExt : OptionM Term → OptionM Term → OptionM Term :=
+-- If terms are well-typed, construct their BV sign extend application
+def mkBvSignExt : Option term → Option term → Option term :=
   λ ot oi => ot >>= λ t => sortOf t >>= λ s =>
              oi >>= λ i => sortOf i >>= λ si =>
   match s, si with
-  | bv n, intSort =>
+  | bv n, intSort => 
     match i with
-    | val (Value.integer i₁) intSort => bvSignExt n (Int.toNat i₁) t i
+    | val (value.integer i₁) intSort => bvSignExt n (Int.toNat i₁) t i
     | _ => none
   | _, _ => none
 
-def hd : List α → OptionM α
+def hd : List α → Option α
 | h :: t => some h
 | [] => none
 
 /-
-If Terms are well-typed, construct their bit-blasted BV sign extend
+If terms are well-typed, construct their bit-blasted BV sign extend
      [x₀ x₁ ... xₙ]    i
 -----------------------------
   [x₀ ... x₀ x₀ x₁ ... xₙ]
 where i x₀'s are prefixed to x
 -/
-def bblastSignExt : OptionM Term → OptionM Term → OptionM Term :=
+def bblastSignExt : Option term → Option term → Option term :=
   λ ot oi => ot >>= λ t => sortOf t >>= λ s =>
              oi >>= λ i => sortOf i >>= λ si =>
   match s, si with
-  | bv n, intSort =>
+  | bv n, intSort => 
     match i with
-    | val (Value.integer i₁) intSort =>
+    | val (value.integer i₁) intSort =>
       match hd (bitOfN t n) with
       | some sign => mkBbT (List.append (List.replicate (Int.toNat i₁) sign) (bitOfN t n))
       | none => none
     | _ => none
   | _, _ => none
-#check bblastSignExt (val (Value.bitvec [true, true, true, true]) (bv 4))
-  (val (Value.integer 2) intSort)
-#check bblastSignExt (val (Value.bitvec [false, true, true, true]) (bv 4))
-  (val (Value.integer 2) intSort)
-#check bblastSignExt (val (Value.bitvec [true, false]) (bv 2))
-  (val (Value.integer 0) intSort)
+#eval bblastSignExt (val (value.bitvec [true, true, true, true]) (bv 4))
+  (val (value.integer 2) intSort)
+#eval bblastSignExt (val (value.bitvec [false, true, true, true]) (bv 4))
+  (val (value.integer 2) intSort)
+#eval bblastSignExt (val (value.bitvec [true, false]) (bv 2))
+  (val (value.integer 0) intSort)
 -- Using variables
-#check bblastSignExt (const (mkName "x") (bv 4)) (val (Value.integer 2) intSort)
+#eval bblastSignExt (const 21 (bv 4)) (val (value.integer 2) intSort)
 
 -- Bit-blasting BvSignExt rule
-axiom bbBvSignExt : ∀ {t₁ t₂ : OptionM Term},
+axiom bbBvSignExt : ∀ {t₁ t₂ : Option term},
   thHolds (mkEq (mkBvSignExt t₁ t₂) (bblastSignExt t₁ t₂))
 
-end Term
+
+end term
 
 end proof
