lean4/Cdclt/Boolean.lean
@@ -1,18 +1,15 @@
 import Cdclt.Term
 
 open proof
-open proof.sort proof.Term
+open proof.sort proof.term
 open List
 
 namespace rules
 
-notation "clause" => List (OptionM Term)
-
-instance : BEq (OptionM Term) :=
- ⟨λ a b => do decide ((← a) = (← b))⟩
+notation "clause" => List (Option term)
 
 -- clause manipulation rules
-def join : OptionM (OptionM α) → OptionM α
+def join : Option (Option α) → Option α
 | some t => t
 | _ => none
 
@@ -20,10 +17,10 @@ universes u v w
 def comp {α : Sort u} {β : Sort v} {φ : Sort w}
   (f : β → φ) (g : α → β) : α → φ := fun x => f (g x)
 
-def nTh : clause → Nat → OptionM Term :=
-  λ c n => join (@List.get? (OptionM Term) n c)
-def getLast : clause → OptionM Term := λ c => nTh c (c.length - 1)
-def concatCl : clause → clause → clause := @List.append (OptionM Term)
+def nTh : clause → Nat → Option term :=
+  λ c n => join (@List.get? (Option term) n c)
+def getLast : clause → Option term := λ c => nTh c (c.length - 1)
+def concatCl : clause → clause → clause := @List.append (Option term)
 def removeDuplicates : clause → clause
 | [] => []
 | (h::t) => if elem h t then removeDuplicates t else h::(removeDuplicates t)
@@ -31,45 +28,45 @@ def removeDuplicates : clause → clause
 
 -- eventually should give Prop
 axiom holds : clause → Type
-axiom thHolds : OptionM Term → Type
+axiom thHolds : Option term → Type
 
--- collect all Terms in OR chain (right-associative)
-def reduceOrAux : Term → clause
-| Term.or t₀ (Term.or t₁ t₂) => t₀::t₁::(reduceOrAux t₂)
-| Term.or t₀ t₁              => [t₀, t₁]
+-- collect all terms in OR chain (right-associative)
+def reduceOrAux : term → clause
+| term.or t₀ (term.or t₁ t₂) => t₀::t₁::(reduceOrAux t₂)
+| term.or t₀ t₁              => [t₀, t₁]
 | t                          => [t]
-def reduceOr : OptionM Term → clause
+def reduceOr : Option term → clause
 | some t => reduceOrAux t
 | none   => [none]
 
 ------------------------------- Clausal Reasoning -------------------------------
 
-def resolveR₀ (n : OptionM Term) (c₁ c₂: clause) : clause :=
+def resolveR₀ (n : Option term) (c₁ c₂: clause) : clause :=
   concatCl (List.erase c₁ n) (List.erase c₂ (mkNot n) )
 
-def resolveR₁ (n : OptionM Term) (c₁ c₂: clause) : clause :=
+def resolveR₁ (n : Option term) (c₁ c₂: clause) : clause :=
   concatCl (List.erase c₁ (mkNot n)) (List.erase c₂ n)
 
 axiom R0 : ∀ {c₁ c₂ : clause},
-  holds c₁ → holds c₂ → (n : OptionM Term) → holds (resolveR₀ n c₁ c₂)
+  holds c₁ → holds c₂ → (n : Option term) → holds (resolveR₀ n c₁ c₂)
 
 axiom R1 : ∀ {c₁ c₂ : clause},
-  holds c₁ → holds c₂ → (n : OptionM Term) → holds (resolveR₁ n c₁ c₂)
+  holds c₁ → holds c₂ → (n : Option term) → holds (resolveR₁ n c₁ c₂)
 
 axiom factoring : ∀ {c : clause}, holds c → holds (removeDuplicates c)
 
 axiom reorder {c₁ : clause} (perm : List Nat) :
   holds c₁ → holds (List.map (nTh c₁) perm)
 
-axiom eqResolve : ∀ {t₁ t₂ : OptionM Term},
+axiom eqResolve : ∀ {t₁ t₂ : Option term},
   thHolds t₁ → thHolds (mkEq t₁ t₂) → thHolds t₂
 
-axiom modusPonens : ∀ {t₁ t₂ : OptionM Term},
+axiom modusPonens : ∀ {t₁ t₂ : Option term},
   thHolds t₁ → thHolds (mkImplies t₁ t₂) → thHolds t₂
 
-axiom notNotElim : ∀ {t : OptionM Term}, thHolds (mkNot $ mkNot t) → thHolds t
+axiom notNotElim : ∀ {t : Option term}, thHolds (mkNot $ mkNot t) → thHolds t
 
-axiom contradiction : ∀ {t : OptionM Term},
+axiom contradiction : ∀ {t : Option term},
   thHolds t → thHolds (mkNot t) → holds []
 
 
@@ -81,14 +78,14 @@ l₁ ∧ ... ∧ lₙ
       lᵢ
 -/
 -- get n-th element in AND chain (right-associative)
-def reduceAndNth : Nat → Term → OptionM Term
-| 0,     (Term.and t v)                 => t
-| 1,     (Term.and _ t)                 => t
-| (n+1), (Term.and  _ (Term.and t₀ t₁)) =>  reduceAndNth n (and t₀ t₁)
+def reduceAndNth : Nat → term → Option term
+| 0,     (term.and t v)                 => t
+| 1,     (term.and _ t)                 => t
+| (n+1), (term.and  _ (term.and t₀ t₁)) =>  reduceAndNth n (and t₀ t₁)
 | _,     _                              => none
-def reduceAnd (n : Nat) : OptionM Term → OptionM Term :=
+def reduceAnd (n : Nat) : Option term → Option term :=
   λ t => t >>= λ t' => reduceAndNth n t'
-axiom andElim : ∀ {t : OptionM Term},
+axiom andElim : ∀ {t : Option term},
   thHolds t → (n : Nat) → thHolds (reduceAnd n t)
 
 /-
@@ -96,7 +93,7 @@ l₁  ...  lₙ
 -----------andIntro
 l₁ ∧ ... ∧ lₙ
 -/
-axiom andIntro : ∀ {t₁ t₂ : OptionM Term},
+axiom andIntro : ∀ {t₁ t₂ : Option term},
   thHolds t₁ → thHolds t₂ → thHolds (mkAnd t₁ t₂)
 
 /-
@@ -105,27 +102,27 @@ axiom andIntro : ∀ {t₁ t₂ : OptionM Term},
         lᵢ
 -/
 -- get n-th in NOT-OR chain (right-associative)
-def reduceOrNth : Nat → Term → OptionM Term
-| 0,     (Term.or t _)               => t
-| 1,     (Term.or _ t)               => t
-| (n+1), (Term.or _ (Term.or t₀ t₁)) => reduceOrNth n (or t₀ t₁)
+def reduceOrNth : Nat → term → Option term
+| 0,     (term.or t _)               => t
+| 1,     (term.or _ t)               => t
+| (n+1), (term.or _ (term.or t₀ t₁)) => reduceOrNth n (or t₀ t₁)
 | _,     _                           => none
 
-def reduceNotOr (n : Nat) (t : OptionM Term) : OptionM Term :=
+def reduceNotOr (n : Nat) (t : Option term) : Option term :=
   t >>= λ t' =>
     match t' with
-    | Term.not t'' => mkNot $ reduceOrNth n t''
+    | term.not t'' => mkNot $ reduceOrNth n t''
     | _            => none
-axiom notOrElim : ∀ {t : OptionM Term} (p : thHolds t) (n : Nat),
+axiom notOrElim : ∀ {t : Option term} (p : thHolds t) (n : Nat),
   thHolds (reduceNotOr n t)
 
-axiom impliesElim : ∀ {t₁ t₂ : OptionM Term},
+axiom impliesElim : ∀ {t₁ t₂ : Option term},
   thHolds (mkImplies t₁ t₂) → holds [mkNot t₁, t₂]
 
-axiom notImplies1 : ∀ {t₁ t₂ : OptionM Term},
+axiom notImplies1 : ∀ {t₁ t₂ : Option term},
   thHolds (mkNot $ mkImplies t₁ t₂) → thHolds t₁
 
-axiom notImplies2 : ∀ {t₁ t₂ : OptionM Term},
+axiom notImplies2 : ∀ {t₁ t₂ : Option term},
   thHolds (mkNot $ mkImplies t₁ t₂) → thHolds (mkNot t₁)
 
 axiom equivElim1 : ∀ {t₁ t₂},
@@ -140,28 +137,28 @@ axiom notEquivElim1 : ∀ {t₁ t₂},
 axiom notEquivElim2 : ∀ {t₁ t₂},
   thHolds (mkNot $ mkEq t₁ t₂) → holds [mkNot t₁, mkNot t₂]
 
-axiom xorElim1 : ∀ {t₁ t₂ : OptionM Term},
+axiom xorElim1 : ∀ {t₁ t₂ : Option term},
   thHolds (mkXor t₁ t₂) → holds [t₁, t₂]
 
-axiom xorElim2 : ∀ {t₁ t₂ : OptionM Term},
+axiom xorElim2 : ∀ {t₁ t₂ : Option term},
   thHolds (mkXor t₁ t₂) → holds [mkNot t₁, mkNot t₂]
 
-axiom notXorElim1 : ∀ {t₁ t₂ : OptionM Term},
+axiom notXorElim1 : ∀ {t₁ t₂ : Option term},
   thHolds (mkNot $ mkXor t₁ t₂) → holds [t₁, mkNot t₂]
 
-axiom notXorElim2 : ∀ {t₁ t₂ : OptionM Term},
+axiom notXorElim2 : ∀ {t₁ t₂ : Option term},
   thHolds (mkNot $ mkXor t₁ t₂) → holds [mkNot t₁, t₂]
 
-axiom iteElim1 : ∀ {c t₁ t₂ : OptionM Term}, thHolds (mkIte c t₁ t₂) →
+axiom iteElim1 : ∀ {c t₁ t₂ : Option term}, thHolds (mkIte c t₁ t₂) →
   holds [mkNot c, t₁]
 
-axiom iteElim2 : ∀ {c t₁ t₂ : OptionM Term}, thHolds (mkIte c t₁ t₂) →
+axiom iteElim2 : ∀ {c t₁ t₂ : Option term}, thHolds (mkIte c t₁ t₂) →
   holds [c, t₂]
 
-axiom notIteElim1 : ∀ {c t₁ t₂ : OptionM Term},
+axiom notIteElim1 : ∀ {c t₁ t₂ : Option term},
   thHolds (mkNot $ mkIte c t₁ t₂) → holds [mkNot c, mkNot t₁]
 
-axiom notIteElim2 : ∀ {c t₁ t₂ : OptionM Term},
+axiom notIteElim2 : ∀ {c t₁ t₂ : Option term},
   thHolds (mkNot $ mkIte c t₁ t₂) → holds [c, mkNot t₂]
 
 /-
@@ -169,14 +166,14 @@ axiom notIteElim2 : ∀ {c t₁ t₂ : OptionM Term},
 ----------------notAnd
 ¬l₁ ∨ ... ∨ ¬lₙ
 -/
-def reduceNotAndAux : Term → clause
-| Term.and t₀ (Term.and t₁ t₂) => mkNot t₀ :: mkNot t₁ :: reduceNotAndAux t₂
-| Term.and t₀ t₁               => [mkNot t₀, mkNot t₁]
+def reduceNotAndAux : term → clause
+| term.and t₀ (term.and t₁ t₂) => mkNot t₀ :: mkNot t₁ :: reduceNotAndAux t₂
+| term.and t₀ t₁               => [mkNot t₀, mkNot t₁]
 | t                            => [t]
-def reduceNotAnd : OptionM Term → clause
+def reduceNotAnd : Option term → clause
 | (some t) => reduceNotAndAux t
 | none     => [none]
-axiom notAnd : ∀ {t : OptionM Term},
+axiom notAnd : ∀ {t : Option term},
   thHolds (mkNot t) → holds (reduceNotAnd t)
 
 
@@ -207,11 +204,11 @@ t₁ → t₂  t₁                 ¬(t₁ → t₂)                ¬(t₁ →
 -----------cnfImpliesPos    ----------cnfImpliesNeg1  ----------cnfImpliesNeg2
      t₂                         t₁                        ¬t₂
 -/
-axiom cnfImpliesPos {t₁ t₂ : OptionM Term} :
+axiom cnfImpliesPos {t₁ t₂ : Option term} :
   holds [mkNot $ mkImplies t₁ t₂, mkNot t₁, t₂]
-axiom cnfImpliesNeg1 {t₁ t₂ : OptionM Term} :
+axiom cnfImpliesNeg1 {t₁ t₂ : Option term} :
 holds [mkImplies t₁ t₂, t₁]
-axiom cnfImpliesNeg2 {t₁ t₂ : OptionM Term} :
+axiom cnfImpliesNeg2 {t₁ t₂ : Option term} :
   holds [mkImplies t₁ t₂, mkNot t₂]
 
 /-
@@ -219,9 +216,9 @@ t₁ = t₂  ¬t₁              t₁ = t₂  t₁
 ------------cnfEquivPos1  ------------cnfEquivPos2
     ¬t₂                        t₂
 -/
-axiom cnfEquivPos1 {t₁ t₂ : OptionM Term} :
+axiom cnfEquivPos1 {t₁ t₂ : Option term} :
   holds [mkNot $ mkEq t₁ t₂, t₁, mkNot t₂]
-axiom cnEquivPos2 {t₁ t₂ : OptionM Term} :
+axiom cnEquivPos2 {t₁ t₂ : Option term} :
   holds [mkNot $ mkEq t₁ t₂, mkNot t₁, t₂]
 
 /-
@@ -229,9 +226,9 @@ axiom cnEquivPos2 {t₁ t₂ : OptionM Term} :
 --------------cnfEquivNeg1  --------------cnfEquivPos2
       ¬t₂                         t₂
 -/
-axiom cnfEquivNeg1 {t₁ t₂ : OptionM Term} :
+axiom cnfEquivNeg1 {t₁ t₂ : Option term} :
   holds [mkEq t₁ t₂, mkNot t₁, mkNot t₂]
-axiom cnfEquivNeg2 {t₁ t₂ : OptionM Term} :
+axiom cnfEquivNeg2 {t₁ t₂ : Option term} :
   holds [mkEq t₁ t₂, t₁, t₂]
 
 /-
@@ -239,9 +236,9 @@ t₁ ⊕ t₂  ¬t₁              t₁ ⊕ t₂  t₁
 ------------cnfXorPos1    -----------cnfXorPos2
      t₂                        ¬t₂
 -/
-axiom cnfXorPos1 {t₁ t₂ : OptionM Term} :
+axiom cnfXorPos1 {t₁ t₂ : Option term} :
   holds [mkNot $ mkXor t₁ t₂, t₁, t₂]
-axiom cnfXorPos2 {t₁ t₂ : OptionM Term} :
+axiom cnfXorPos2 {t₁ t₂ : Option term} :
   holds [mkNot $ mkXor t₁ t₂, mkNot t₁, mkNot t₂]
 
 /-
@@ -249,9 +246,9 @@ axiom cnfXorPos2 {t₁ t₂ : OptionM Term} :
 ---------------cnfXorNeg1  --------------cnfXorNeg2
       ¬t₂                        ¬t₂
 -/
-axiom cnfXorNeg1 {t₁ t₂ : OptionM Term} :
+axiom cnfXorNeg1 {t₁ t₂ : Option term} :
   holds [mkXor t₁ t₂, t₁, mkNot t₂]
-axiom cnfXorNeg2 {t₁ t₂ : OptionM Term} :
+axiom cnfXorNeg2 {t₁ t₂ : Option term} :
   holds [mkXor t₁ t₂, mkNot t₁, t₂]
 
 /-
@@ -263,11 +260,11 @@ ite c t₁ t₂  ¬t₁
 ----------------cnfItePos3
         t₂
 -/
-axiom cnfItePos1 {c t₁ t₂ : OptionM Term} :
+axiom cnfItePos1 {c t₁ t₂ : Option term} :
   holds [mkNot $ mkIte c t₁ t₂, mkNot c, t₁]
-axiom cnfItePos2 {c t₁ t₂ : OptionM Term} :
+axiom cnfItePos2 {c t₁ t₂ : Option term} :
   holds [mkNot $ mkIte c t₁ t₂, c, t₂]
-axiom cnfItePos3 {c t₁ t₂ : OptionM Term} :
+axiom cnfItePos3 {c t₁ t₂ : Option term} :
   holds [mkNot $ mkIte c t₁ t₂, t₁, t₂]
 
 /-
@@ -280,30 +277,30 @@ axiom cnfItePos3 {c t₁ t₂ : OptionM Term} :
 ------------------cnfIteNeg3
         ¬t₂
 -/
-axiom cnfIteNeg1 {c t₁ t₂ : OptionM Term} :
+axiom cnfIteNeg1 {c t₁ t₂ : Option term} :
   holds [mkIte c t₁ t₂, c, mkNot t₁]
-axiom cnfIteNeg2 {c t₁ t₂ : OptionM Term} :
+axiom cnfIteNeg2 {c t₁ t₂ : Option term} :
   holds [mkIte c t₁ t₂, mkNot c, mkNot t₂]
-axiom cnfIteNeg3 {c t₁ t₂ : OptionM Term} :
+axiom cnfIteNeg3 {c t₁ t₂ : Option term} :
   holds [mkIte c t₁ t₂, mkNot t₁, mkNot t₂]
 
 -- connecting theory reasoning and clausal reasoning
 ---------------- Connecting Theory Reasoning and Clausal Reasoning ----------------
-axiom thAssume : ∀ {t : OptionM Term}, holds [t] → thHolds t
+axiom thAssume : ∀ {t : Option term}, holds [t] → thHolds t
 
-axiom clAssume : ∀ {t : OptionM Term}, thHolds t → holds [t]
+axiom clAssume : ∀ {t : Option term}, thHolds t → holds [t]
 
-axiom clOr : ∀ {t : OptionM Term} (p : thHolds t), holds (reduceOr t)
+axiom clOr : ∀ {t : Option term} (p : thHolds t), holds (reduceOr t)
 
-axiom scope : ∀ {t₁ t₂ : OptionM Term},
+axiom scope : ∀ {t₁ t₂ : Option term},
   thHolds t₁ → thHolds t₂ → thHolds (mkOr (mkNot t₁) t₂)
 
 ------------------------------------ Holes ------------------------------------
 
 axiom trust : ∀ {c₁ c₂ : clause}, holds c₁ → holds c₂
 
-axiom thTrust : ∀ {t₁ t₂ : OptionM Term}, thHolds t₁ → thHolds t₂
+axiom thTrust : ∀ {t₁ t₂ : Option term}, thHolds t₁ → thHolds t₂
 
-axiom thTrustValid : ∀ {t : OptionM Term}, thHolds t
+axiom thTrustValid : ∀ {t : Option term}, thHolds t
 
 end rules
